Refactor DEFINE-COPY

books/projects/atomic-stobjs/constructors/copy.lisp
@@ -64,9 +64,9 @@
 (defmacro coupledp (&rest names)
   (declare (xargs :guard (symbol-listp names)))
   (let ((expressions (coupledp-fn names ())))
-    (list 'case-split (if (endp (cdr expressions))
-                          (car expressions)
-                          (cons 'and expressions)))))
+    (list 'force (if (endp (cdr expressions))
+                     (car expressions)
+                     (cons 'and expressions)))))
 
 
 ;;;; `MAKE-VECTOR-COPY-EVENTS'
@@ -79,16 +79,16 @@
   (let* ((%vector (symbolicate package-witness "%" vector))
          (copy (symbolicate package-witness vector "-COPY"))
          (copy-rec (symbolicate package-witness copy "-REC"))
-         (copy-rw (symbolicate package-witness copy "-RW"))
          (index (symbolicate package-witness "I"))
 
          (coupledp (symbolicate package-witness vector "-COUPLED-P"))
          (coupledp-witness (symbolicate package-witness coupledp "-WITNESS"))
+         (coupledp-necc (symbolicate package-witness coupledp "-NECC"))
 
          ;; `VECTOR'
          (stobj-property (getpropc vector 'acl2::stobj))
          (recognizer (caadr stobj-property))
-         (fixer (first (third stobj-property)))
+         (the-vector (symbolicate vector "THE-" vector))
          (length (second (third stobj-property)))
          (resizer (third (third stobj-property)))
          (accessor (fourth (third stobj-property)))
@@ -99,12 +99,13 @@
          (stobj$a-property (cdr (assoc vector (table-alist 'stobj$a-property world))))
          (vector$a (first stobj$a-property))
          (recognizer$a-aux (symbolicate vector$a vector$a "-AUX-P"))
-         (vector$a-definitions (symbolicate vector$a vector$a "-DEFINITIONS"))
          (vector$a-theorems (symbolicate vector$a vector$a "-THEOREMS"))
          (vector$a-aggressive (symbolicate vector$a vector$a "-AGGRESSIVE"))
+         (vector$a-constraints (symbolicate vector$a vector$a "-CONSTRAINTS"))
          (recognizer$a (first (second stobj$a-property)))
          (creator$a (second (second stobj$a-property)))
          (fixer$a (third (second stobj$a-property)))
+         (equiv$a (fourth (second stobj$a-property)))
          (resizable (first (second (third stobj$a-property))))
          (default-length-name (second (second (third stobj$a-property))))
          (length$a (first (third (third stobj$a-property))))
@@ -113,6 +114,7 @@
          (updater$a (fourth (third (third stobj$a-property))))
 
          (element (first (first (third stobj$a-property))))
+         (%element (symbolicate element "%" element))
          (element-stobj-property (getpropc element 'acl2::stobj))
          (element-stobj$a-property (cdr (assoc element (table-alist 'stobj$a-property world))))
          (element-recognizer (second (first (third stobj$a-property))))
@@ -122,11 +124,9 @@
                               `(,element-creator)
                               initial-element-name))
          (element-fixer (fourth (first (third stobj$a-property))))
+         (element-equiv (fifth (first (third stobj$a-property))))
 
          ;; Adjust for nested stobj interface shuffle
-         (fixer (if element-stobj-property
-                    (third (third stobj-property))
-                    fixer))
          (length (if element-stobj-property
                      (fourth (third stobj-property))
                      length))
@@ -144,7 +144,6 @@
 
          (element-copy (cdr (assoc element (table-alist 'copy world))))
          (element-copy-theory (symbolicate element-copy element-copy "-THEORY"))
-         (%element (car (getpropc element-copy 'acl2::formals)))
          (element-coupled-p (cdr (assoc element (table-alist 'coupledp world))))
 
          (copy-begin (symbolicate package-witness copy "-BEGIN"))
@@ -152,29 +151,32 @@
          (copy-theory (symbolicate package-witness copy "-THEORY"))
 
          ;; Theorem Names
-         (booleanp-of-element-recognizer (symbolicate "ATOMIC-STOBJS" "BOOLEANP-OF-" element-recognizer))
-         (element-recognizer-of-initial-element (symbolicate "ATOMIC-STOBJS" element-recognizer "-OF-INITIAL-ELEMENT"))
-         (element-fixer-rw (symbolicate "ATOMIC-STOBJS" element-fixer "-RW"))
+         (element-recognizer-constraints (symbolicate "ATOMIC-STOBJS" element-recognizer "-CONSTRAINTS"))
+         (element-fixer-constraints (symbolicate "ATOMIC-STOBJS" element-fixer "-CONSTRAINTS"))
+         (element-equiv-constraints (symbolicate "ATOMIC-STOBJS" element-equiv "-CONSTRAINTS"))
 
-         (coupledp-constraint-1 (symbolicate "ATOMIC-STOBJS" coupledp "-CONSTRAINT-1"))
-         (coupledp-constraint-2 (symbolicate "ATOMIC-STOBJS" coupledp "-CONSTRAINT-2"))
-         (coupledp-constraint-1/expanded (symbolicate "ATOMIC-STOBJS" coupledp-constraint-1 "/EXPANDED"))
-         (coupledp-constraint-2/expanded (symbolicate "ATOMIC-STOBJS" coupledp-constraint-2 "/EXPANDED"))
-
-         (copy-rec-of-fixer$a-3 (symbolicate "ATOMIC-STOBJS" copy-rec "-OF-" fixer$a "-3"))
-         (copy-rec-constraint (symbolicate "ATOMIC-STOBJS" copy-rec "-CONSTRAINT"))
-
+         (coupledp-constraints (symbolicate package-witness coupledp "-CONSTRAINTS"))
+         (coupledp-tp (symbolicate package-witness coupledp "-TP"))
          (coupledp-when-not-recognizer$a (symbolicate package-witness coupledp "-WHEN-NOT-" recognizer$a))
          (coupledp-of-creator$a (symbolicate package-witness coupledp "-OF-" creator$a))
-         (coupledp-of-fixer$a (symbolicate package-witness coupledp "-OF-" fixer$a))
          (coupledp-of-resizer$a (symbolicate package-witness coupledp "-OF-" resizer$a))
          (element-coupled-p-of-accessor$a (symbolicate package-witness element-coupled-p "-OF-" accessor$a))
          (coupledp-of-updater$a (symbolicate package-witness coupledp "-OF-" updater$a))
 
+         (copy-rec-of-fixer$a-2 (symbolicate "ATOMIC-STOBJS" copy-rec "-OF-" fixer$a "-2"))
+         (copy-rec-of-fixer$a-3 (symbolicate "ATOMIC-STOBJS" copy-rec "-OF-" fixer$a "-3"))
+
+         (vector-copy-constraints (symbolicate package-witness copy "-CONSTRAINTS"))
          (recognizer$a-of-copy (symbolicate package-witness recognizer$a "-OF-" copy))
          (copy-ignores-1 (symbolicate package-witness copy "-IGNORES-1"))
-         (copy-of-fixer$a-2 (symbolicate package-witness copy "-OF-" fixer$a "-2"))
+         (coupledp-of-copy (symbolicate package-witness coupledp "-OF-" copy))
          (length$a-of-copy (symbolicate package-witness length$a "-OF-" copy))
+         (copy-of-resizer$a (symbolicate package-witness copy "-OF-" resizer$a))
+         (accessor$a-of-copy (symbolicate package-witness accessor$a "-OF-" copy))
+         (accessor$a-of-copy-lemma (symbolicate "ATOMIC-STOBJS" accessor$a-of-copy "-LEMMA"))
+         (copy-of-updater$a (symbolicate package-witness copy "-OF-" updater$a))
+         (copy-of-updater$a-lemma (symbolicate "ATOMIC-STOBJS" copy-of-updater$a "-LEMMA"))
+         (copy-rw (symbolicate package-witness copy "-RW"))
 
          (fi-bindings
           (append
@@ -207,11 +209,14 @@
                  `(lem-vector$a::element-fixer ,(or element-fixer
                                                     '(lambda (element)
                                                       element)))
-                 `(lem-vector$a::contents-recognizer ,(if element-recognizer
-                                                          (if resizable
-                                                              recognizer$a
-                                                              recognizer$a-aux)
-                                                          'true-listp))
+                 `(lem-vector$a::element-equiv ,(or element-equiv
+                                                    'equal))
+
+                 `(lem-vector$a::recognizer-aux ,(if element-recognizer
+                                                     (if resizable
+                                                         recognizer$a
+                                                         recognizer$a-aux)
+                                                     'true-listp))
                  (if resizable
                      `(lem-vector$a::recognizer/resizable ,recognizer$a)
                      `(lem-vector$a::recognizer/fixed ,recognizer$a))
@@ -219,6 +224,9 @@
                  (if resizable
                      `(lem-vector$a::fixer/resizable ,fixer$a)
                      `(lem-vector$a::fixer/fixed ,fixer$a))
+                 (if resizable
+                     `(lem-vector$a::equiv/resizable ,equiv$a)
+                     `(lem-vector$a::equiv/fixed ,equiv$a))
                  (if resizable
                      `(lem-vector$a::length/resizable ,length$a)
                      `(lem-vector$a::length/fixed ,length$a))
@@ -257,26 +265,32 @@
          (local
            (deflabel prologue-begin))
 
-         ,@(and element-recognizer
-                element-fixer
+         ,@(and element-fixer
+                element-recognizer
+                (not (eq element-equiv 'equal))
                 `((local
-                    (defthm ,booleanp-of-element-recognizer
-                      (booleanp (,element-recognizer ,element))
+                    (defthm ,element-recognizer-constraints
+                      (and (booleanp (,element-recognizer ,element))
+                           (,element-recognizer ,initial-element))
                       :rule-classes
-                      (:rewrite
-                       :type-prescription)))
+                      ((:rewrite :corollary
+                                 (booleanp (,element-recognizer ,element)))
+                       ,@(and (not (equal initial-element initial-element-name))
+                              `((:rewrite :corollary
+                                          (,element-recognizer ,initial-element)))))))
 
                   (local
-                    (defthm ,element-recognizer-of-initial-element
-                      (,element-recognizer ,initial-element)
-                      :rule-classes nil))
-
-                  (local
-                    (defthm ,element-fixer-rw
+                    (defthm ,element-fixer-constraints
                       (equal (,element-fixer ,element)
                              (if (,element-recognizer ,element)
                                  ,element
-                                 ,initial-element))))))
+                                 ,initial-element))))
+
+                  (local
+                    (defthm ,element-equiv-constraints
+                      (equal (,element-equiv ,%element ,element)
+                             (equal (,element-fixer ,%element)
+                                    (,element-fixer ,element)))))))
 
          (local
            (deflabel prologue-end))
@@ -290,10 +304,14 @@
          (local
            (in-theory
              (union-theories
-              (union-theories (theory 'acl2::ground-zero)
-                              (theory ',vector$a-definitions))
+              (theory 'acl2::ground-zero)
               (set-difference-theories (current-theory 'prologue-end)
                                        (current-theory 'prologue-begin)))))
+
+         ,@(and element-copy
+                `((local
+                    (in-theory
+                      (enable ,element-copy-theory)))))
 
          (local
            (in-theory
@@ -301,23 +319,9 @@
                       (:e make-list-ac))))
 
          ,@(and element-recognizer
-                element-fixer
                 `((local
                     (in-theory
-                      (e/d ((:e ,element-recognizer)
-                            (:e ,element-fixer))
-                           (,element-recognizer
-                            ,element-fixer))))))
-
-         ,@(and element-stobj$a-property
-                `((local
-                    (in-theory
-                      (disable ,element-creator)))))
-
-         ,@(and element-stobj-property
-                `((local
-                    (in-theory
-                      (enable ,element-copy-theory)))))
+                      (enable (:e ,element-recognizer))))))
 
          ,@(and element-stobj-property
                 `((local
@@ -332,10 +336,6 @@
            :package-witness ,package-witness
            :debug ,debug)
 
-         (local
-           (in-theory
-             (enable ,@(strip-cars (cdr (getpropc %vector 'acl2::absstobj-info))))))
-
          ;; `COUPLEDP'
          ,@(and element-coupled-p
                 `((defun-sk ,coupledp (,vector)
@@ -347,98 +347,76 @@
 
                   (table coupledp ',vector ',coupledp)
 
-                  (local
-                    (defthmd ,coupledp-constraint-1
-                      (implies (,coupledp ,vector)
-                               (,element-coupled-p (,accessor$a ,index ,vector)))
-                      :hints
-                      (("Goal"
-                        :in-theory (disable ,coupledp
-                                            ,vector$a-definitions)))))
+                  (defthm ,coupledp-constraints
+                    (and (equal (,coupledp ,vector)
+                                ((lambda (,index ,vector)
+                                   (,element-coupled-p (,accessor$a ,index ,vector)))
+                                 (,coupledp-witness ,vector)
+                                 ,vector))
+                         (implies (,coupledp ,vector)
+                                  (,element-coupled-p (,accessor$a ,index ,vector))))
+                    :rule-classes
+                    ((:definition :corollary
+                         (equal (,coupledp ,vector)
+                                ((lambda (,index ,vector)
+                                   (,element-coupled-p (,accessor$a ,index ,vector)))
+                                 (,coupledp-witness ,vector)
+                                 ,vector)))
+                     (:rewrite :corollary
+                               (implies (,coupledp ,vector)
+                                        (,element-coupled-p (,accessor$a ,index ,vector)))))
+                    :hints
+                    (("Goal"
+                      :in-theory (disable ,coupledp-necc)
+                      :use ((:instance ,coupledp-necc)))))
 
                   (local
-                    (defthmd ,coupledp-constraint-2
-                      (equal (,coupledp ,vector)
-                             ((lambda (,index ,vector)
-                                (,element-coupled-p (,accessor$a ,index ,vector)))
-                              (,coupledp-witness ,vector) ,vector))))
+                    (in-theory
+                      (disable ,coupledp
+                               (:definition ,coupledp-constraints))))
 
-                  (in-theory
-                    (disable ,coupledp))
-
-                  (local
-                    (defthmd ,coupledp-constraint-1/expanded
-                      (implies (,coupledp ,vector)
-                               (,element-coupled-p (let ((,index (nfix ,index))
-                                                         (,vector (,fixer$a ,vector)))
-                                                     (if (< ,index ,(if resizable
-                                                                        `(len (,fixer$a ,vector))
-                                                                        default-length-name))
-                                                         (,element-fixer (nth ,index ,vector))
-                                                         (,element-creator)))))
-                      :hints
-                      (("Goal"
-                        :in-theory (e/d (,vector$a-theorems)
-                                        (,vector$a-definitions
-                                         nfix))
-                        :use ,coupledp-constraint-1
-                        :expand ((:free (,index ,vector)
-                                        (,accessor$a ,index ,vector))
-                                 (:free (,vector)
-                                        (,length$a ,vector)))))))
-
-                  (local
-                    (defthmd ,coupledp-constraint-2/expanded
-                      (equal (,coupledp ,vector)
-                             (,element-coupled-p (let ((,index (nfix (,coupledp-witness ,vector)))
-                                                       (,vector (,fixer$a ,vector)))
-                                                   (if (< ,index ,(if resizable
-                                                                      `(len (,fixer$a ,vector))
-                                                                      default-length-name))
-                                                       (,element-fixer (nth ,index ,vector))
-                                                       (,element-creator)))))
-                      :hints
-                      (("Goal"
-                        :in-theory (e/d (,vector$a-theorems)
-                                        (,vector$a-definitions
-                                         nfix))
-                        :use ,coupledp-constraint-2
-                        :expand ((:free (,index ,vector)
-                                        (,accessor$a ,index ,vector))
-                                 (:free (,vector)
-                                        (,length$a ,vector)))))))
+                  (defthm ,coupledp-tp
+                    (booleanp (,coupledp ,vector))
+                    :rule-classes :type-prescription
+                    :hints
+                    (("Goal"
+                      :in-theory (enable ,vector$a-theorems)
+                      :by (:functional-instance
+                           ,(if resizable
+                                'lem-vector$a::coupledp/resizable-tp
+                                'lem-vector$a::coupledp/fixed-tp)
+                           ,@fi-bindings))
+                     ("Subgoal 7"
+                      :use ((:instance (:definition ,coupledp-constraints)
+                                       (,vector lem-vector$a::vector))))
+                     ,@(if resizable
+                           `(("Subgoal 6"
+                              :in-theory (enable ,vector$a-constraints))
+                             ("Subgoal 4"
+                              :in-theory (enable ,vector$a-constraints))
+                             ("Subgoal 3"
+                              :in-theory (enable ,vector$a-constraints))
+                             ("Subgoal 1"
+                              :in-theory (enable ,vector$a-constraints)))
+                           `(("Subgoal 6"
+                              :in-theory (enable ,vector$a-constraints))
+                             ("Subgoal 4"
+                              :in-theory (enable ,vector$a-constraints))
+                             ("Subgoal 3"
+                              :in-theory (enable ,vector$a-constraints))
+                             ("Subgoal 2"
+                              :in-theory (enable ,vector$a-constraints))))))
 
                   (defthm ,coupledp-when-not-recognizer$a
                     (implies (not (,recognizer$a ,vector))
                              (,coupledp ,vector))
                     :hints
                     (("Goal"
-                      :do-not-induct t
                       :by (:functional-instance
                            ,(if resizable
                                 'lem-vector$a::coupledp/resizable-when-not-recognizer/resizable
                                 'lem-vector$a::coupledp/fixed-when-not-recognizer/fixed)
-                           ,@fi-bindings))
-                     ,@(and element-coupled-p
-                            (if resizable
-                                `(("Subgoal 6"
-                                   :in-theory (theory 'acl2::minimal-theory)
-                                   :use (:instance ,coupledp-constraint-1/expanded
-                                                   (,index lem-vector$a::index)
-                                                   (,vector common-lisp::vector)))
-                                  ("Subgoal 5"
-                                   :in-theory (theory 'acl2::minimal-theory)
-                                   :use (:instance ,coupledp-constraint-2/expanded
-                                                   (,vector common-lisp::vector))))
-                                `(("Subgoal 7"
-                                   :in-theory (theory 'acl2::minimal-theory)
-                                   :use (:instance ,coupledp-constraint-1/expanded
-                                                   (,index lem-vector$a::index)
-                                                   (,vector common-lisp::vector)))
-                                  ("Subgoal 6"
-                                   :in-theory (theory 'acl2::minimal-theory)
-                                   :use (:instance ,coupledp-constraint-2/expanded
-                                                   (,vector common-lisp::vector))))))))
+                           ,@fi-bindings))))
 
                   (defthm ,coupledp-of-creator$a
                     (,coupledp (,creator$a))
@@ -450,15 +428,14 @@
                                 'lem-vector$a::coupledp/fixed-of-creator)
                            ,@fi-bindings))))
 
-                  (defthm ,coupledp-of-fixer$a
-                    (equal (,coupledp (,fixer$a ,vector))
-                           (,coupledp ,vector))
+                  (defcong ,equiv$a equal (,coupledp ,vector) 1
                     :hints
                     (("Goal"
+                      :in-theory (enable ,equiv$a)
                       :by (:functional-instance
                            ,(if resizable
-                                'lem-vector$a::coupledp/resizable-of-fixer/resizable
-                                'lem-vector$a::coupledp/fixed-of-fixer/fixed)
+                                'lem-vector$a::equiv/resizable-implies-equal-coupledp/resizable-1
+                                'lem-vector$a::equiv/fixed-implies-equal-coupledp/fixed-1)
                            ,@fi-bindings))))
 
                   ,@(and resizable
@@ -467,6 +444,7 @@
                                       (,coupledp (,resizer$a length ,vector)))
                              :hints
                              (("Goal"
+                               :in-theory (enable ,vector$a-constraints)
                                :by (:functional-instance
                                     lem-vector$a::coupledp/resizable-of-resizer/resizable
                                     ,@fi-bindings))))))
@@ -474,10 +452,6 @@
                   (defthm ,element-coupled-p-of-accessor$a
                     (implies (,coupledp ,vector)
                              (,element-coupled-p (,accessor$a ,index ,vector)))
-                    :rule-classes
-                    ((:rewrite :corollary
-                               (implies (coupledp ,vector)
-                                        (,element-coupled-p (,accessor$a ,index ,vector)))))
                     :hints
                     (("Goal"
                       :by (:functional-instance
@@ -489,14 +463,15 @@
                   (defthm ,coupledp-of-updater$a
                     (implies (,coupledp ,vector)
                              (equal (,coupledp (,updater$a ,index ,element ,vector))
-                                    (if (<= ,(if resizable
-                                                 `(,length$a ,vector)
-                                                 default-length-name)
-                                            (nfix ,index))
-                                        t
-                                        (,element-coupled-p ,element))))
+                                    (if (< (nfix ,index)
+                                           ,(if resizable
+                                                `(,length$a ,vector)
+                                                default-length-name))
+                                        (,element-coupled-p ,element)
+                                        t)))
                     :hints
                     (("Goal"
+                      :in-theory (enable ,vector$a-constraints)
                       :by (:functional-instance
                            ,(if resizable
                                 'lem-vector$a::coupledp/resizable-of-updater/resizable
@@ -511,11 +486,10 @@
                                        (<= ,index (,length ,vector)))
                            :guard-hints
                            (("Goal"
-                             :in-theory (e/d (,vector$a-theorems
-                                              ,vector$a-aggressive)
-                                             (,vector$a-definitions))))))
+                             :in-theory (enable ,vector$a-theorems
+                                                ,vector$a-aggressive)))))
            (if (zp ,index)
-               (,fixer ,%vector)
+               (,the-vector ,%vector)
                ,(if element-copy
                     `(let ((,index (1- ,index)))
                        (stobj-let ((,element (,accessor ,index ,vector) ,updater))
@@ -530,68 +504,149 @@
                             (,%vector (,updater ,index ,element ,%vector)))
                        (,copy-rec ,index ,%vector ,vector)))))
 
-         (local
-           (defthm ,copy-rec-of-fixer$a-3
-             (equal (,copy-rec ,index ,%vector (,fixer$a ,vector))
-                    (,copy-rec ,index ,%vector ,vector))
-             :hints
-             (("Goal"
-               :in-theory (e/d (,vector$a-theorems
-                                ,vector$a-aggressive)
-                               (,vector$a-definitions))))))
-
-         (local
-           (defthm ,copy-rec-constraint
-             (equal (,copy-rec ,index ,%vector ,vector)
-                    (if (zp ,index)
-                        (,fixer$a ,%vector)
-                        (let* ((,index (1- ,index))
-                               (element (,accessor$a ,index ,vector))
-                               (%element (,accessor$a ,index ,%vector)))
-                          (declare (ignorable %element))
-                          (let* ((%element ,(cond
-                                              (element-copy
-                                               `(,element-copy %element element))
-                                              (element-fixer
-                                               `(,element-fixer element))
-                                              (t
-                                               'element)))
-                                 (,%vector (,updater$a ,index %element ,%vector))
-                                 (,vector (,updater$a ,index element ,vector)))
-                            (,copy-rec ,index ,%vector ,vector)))))
-             :hints
-             (("Goal"
-               :do-not-induct t
-               :in-theory (e/d (,vector$a-theorems
-                                ,vector$a-aggressive)
-                               (,vector$a-definitions))))))
-
-         (in-theory
-           (disable ,copy-rec))
-
          ;; `COPY'
          (defun ,copy (,%vector ,vector)
            (declare (xargs :stobjs (,%vector ,vector)
                            :guard-hints
                            (("Goal"
-                             :in-theory (e/d (,vector$a-theorems
-                                              ,vector$a-aggressive)
-                                             (,vector$a-definitions))))))
+                             :in-theory (enable ,vector$a-theorems
+                                                ,vector$a-aggressive)))))
            ,(if resizable
                 `(let* ((length (,length ,vector))
                         (,%vector (if (= (,length ,%vector) length)
-                                      ,%vector
+                                      (,the-vector ,%vector)
                                       (,resizer length ,%vector))))
                    (,copy-rec length ,%vector ,vector))
                 `(,copy-rec ,default-length-name ,%vector ,vector)))
 
          (table copy ',vector ',copy)
 
+         (local
+           (defthmd ,copy-rec-of-fixer$a-2
+             (equal (,copy-rec ,index (,fixer$a ,%vector) ,vector)
+                    (,copy-rec ,index ,%vector ,vector))
+             :hints
+             (("Goal"
+               :induct (,copy-rec ,index ,%vector ,vector)
+               :in-theory (enable ,vector$a-theorems)))))
+
+         (local
+           (defthmd ,copy-rec-of-fixer$a-3
+             (equal (,copy-rec ,index ,%vector (,fixer$a ,vector))
+                    (,copy-rec ,index ,%vector ,vector))
+             :hints
+             (("Goal"
+               :induct (,copy-rec ,index ,%vector ,vector)
+               :in-theory (enable ,vector$a-theorems)
+               :expand (,copy-rec ,index ,%vector (,fixer$a ,vector))))))
+
+         (defthm ,vector-copy-constraints
+           (and (equal (,copy-rec ,index ,%vector ,vector)
+                       (if (zp ,index)
+                           (,fixer$a ,%vector)
+                           ((lambda (,index ,%vector ,vector)
+                              ((lambda (,element ,vector ,%vector ,index)
+                                 ((lambda (,%element ,index ,%vector ,vector ,element)
+                                    (declare (ignorable ,%element))
+                                    ((lambda (,%element ,element ,vector ,%vector ,index)
+                                       ((lambda (,%vector ,vector ,element ,index)
+                                          ((lambda (,vector ,%vector ,index)
+                                             (,copy-rec ,index ,%vector ,vector))
+                                           (,updater$a ,index ,element ,vector)
+                                           ,%vector ,index))
+                                        (,updater$a ,index ,%element ,%vector)
+                                        ,vector ,element ,index))
+                                     ,(cond
+                                        (element-copy
+                                         `(,element-copy ,%element ,element))
+                                        (element-fixer
+                                         `(,element-fixer ,element))
+                                        (t
+                                         element))
+                                     ,element ,vector ,%vector ,index))
+                                  (,accessor$a ,index ,%vector)
+                                  ,index ,%vector ,vector ,element))
+                               (,accessor$a ,index ,vector)
+                               ,vector ,%vector ,index))
+                            (binary-+ '-1 ,index)
+                            ,%vector ,vector)))
+                (equal (,copy ,%vector ,vector)
+                       ((lambda (length ,vector ,%vector)
+                          ((lambda (,%vector ,vector length)
+                             (,copy-rec length ,%vector ,vector))
+                           ,(if resizable
+                                `(if (equal (,length$a ,%vector)
+                                            length)
+                                     ,%vector
+                                     (,resizer$a length ,%vector))
+                                %vector)
+                           ,vector length))
+                        (,length$a ,vector)
+                        ,vector ,%vector)))
+           :rule-classes
+           ((:definition :corollary
+                (equal (,copy-rec ,index ,%vector ,vector)
+                       (if (zp ,index)
+                           (,fixer$a ,%vector)
+                           ((lambda (,index ,%vector ,vector)
+                              ((lambda (,element ,vector ,%vector ,index)
+                                 ((lambda (,%element ,index ,%vector ,vector ,element)
+                                    (declare (ignorable ,%element))
+                                    ((lambda (,%element ,element ,vector ,%vector ,index)
+                                       ((lambda (,%vector ,vector ,element ,index)
+                                          ((lambda (,vector ,%vector ,index)
+                                             (,copy-rec ,index ,%vector ,vector))
+                                           (,updater$a ,index ,element ,vector)
+                                           ,%vector ,index))
+                                        (,updater$a ,index ,%element ,%vector)
+                                        ,vector ,element ,index))
+                                     ,(cond
+                                        (element-copy
+                                         `(,element-copy ,%element ,element))
+                                        (element-fixer
+                                         `(,element-fixer ,element))
+                                        (t
+                                         element))
+                                     ,element ,vector ,%vector ,index))
+                                  (,accessor$a ,index ,%vector)
+                                  ,index ,%vector ,vector ,element))
+                               (,accessor$a ,index ,vector)
+                               ,vector ,%vector ,index))
+                            (binary-+ '-1 ,index)
+                            ,%vector ,vector))))
+            (:definition :corollary
+                (equal (,copy ,%vector ,vector)
+                       ((lambda (length ,vector ,%vector)
+                          ((lambda (,%vector ,vector length)
+                             (,copy-rec length ,%vector ,vector))
+                           ,(if resizable
+                                `(if (equal (,length$a ,%vector)
+                                            length)
+                                     ,%vector
+                                     (,resizer$a length ,%vector))
+                                %vector)
+                           ,vector length))
+                        (,length$a ,vector)
+                        ,vector ,%vector))))
+           :hints
+           (("Goal"
+             :do-not-induct t
+             :in-theory (enable ,vector$a-theorems
+                                ,vector$a-aggressive
+                                ,copy-rec-of-fixer$a-3
+                                ,copy-rec-of-fixer$a-2))))
+
+         (local
+           (in-theory
+             (disable ,copy-rec
+                      ,copy)))
+
          (defthm ,recognizer$a-of-copy
            (,recognizer$a (,copy ,%vector ,vector))
            :hints
            (("Goal"
              :do-not-induct t
+             :in-theory (enable ,vector$a-constraints)
              :by (:functional-instance
                   ,(if resizable
                        'lem-vector$a::recognizer/resizable-of-copy/resizable
@@ -615,16 +670,26 @@
                        'lem-vector$a::copy/fixed-ignores-1)
                   ,@fi-bindings-with-copy))))
 
-         (defthm ,copy-of-fixer$a-2
-           (equal (,copy ,%vector (,fixer$a ,vector))
-                  (,copy ,%vector ,vector))
+         (defcong ,equiv$a equal (,copy ,%vector ,vector) 2
            :hints
            (("Goal"
+             :in-theory (enable ,vector$a-constraints)
              :by (:functional-instance
                   ,(if resizable
-                       'lem-vector$a::copy/resizable-of-fixer/resizable-2
-                       'lem-vector$a::copy/fixed-of-fixer/fixed-2)
+                       'lem-vector$a::equiv/resizable-implies-equal-copy/resizable-2
+                       'lem-vector$a::equiv/fixed-implies-equal-copy/fixed-2)
                   ,@fi-bindings-with-copy))))
+
+         ,@(and element-coupled-p
+                `((defthm ,coupledp-of-copy
+                    (,coupledp (,copy ,%vector ,vector))
+                    :hints
+                    (("Goal"
+                      :by (:functional-instance
+                           ,(if resizable
+                                'lem-vector$a::coupledp/resizable-of-copy/resizable
+                                'lem-vector$a::coupledp/fixed-of-copy/fixed)
+                           ,@fi-bindings-with-copy))))))
 
          ,@(and resizable
                 `((defthm ,length$a-of-copy
@@ -634,10 +699,83 @@
                     (("Goal"
                       :by (:functional-instance
                            lem-vector$a::length/resizable-of-copy/resizable
+                           ,@fi-bindings-with-copy))))
+
+                  (defthm ,copy-of-resizer$a
+                    (equal (,copy ,%vector (,resizer$a length ,vector))
+                           (,resizer$a length (,copy ,%vector ,vector)))
+                    :hints
+                    (("Goal"
+                      :by (:functional-instance
+                           lem-vector$a::copy/resizable-of-resizer/resizable
                            ,@fi-bindings-with-copy))))))
 
-         (in-theory
-           (disable ,copy))
+         (local
+           (defthmd ,accessor$a-of-copy-lemma
+             (equal (,accessor$a ,index (,copy ,%vector ,vector))
+                    ,(cond
+                       (element-copy
+                        `(,element-copy ,initial-element (,accessor$a ,index ,vector)))
+                       (element-fixer
+                        `(,element-fixer (,accessor$a ,index ,vector)))
+                       (t
+                        `((lambda (x) x) (,accessor$a ,index ,vector)))))
+             :hints
+             (("Goal"
+               :by (:functional-instance
+                    ,(if resizable
+                         'lem-vector$a::accessor/resizable-of-copy/resizable
+                         'lem-vector$a::accessor/fixed-of-copy/fixed)
+                    ,@fi-bindings-with-copy)))))
+
+         (defthm ,accessor$a-of-copy
+           (equal (,accessor$a ,index (,copy ,%vector ,vector))
+                  ,(if element-copy
+                       `(,element-copy ,initial-element (,accessor$a ,index ,vector))
+                       `(,accessor$a ,index ,vector)))
+           :hints
+           (("Goal"
+             :use ,accessor$a-of-copy-lemma)))
+
+         (local
+           (defthmd ,copy-of-updater$a-lemma
+             (equal (,copy ,%vector (,updater$a ,index ,element ,vector))
+                    (if (< (nfix ,index) ,(if resizable
+                                              `(,length$a ,vector)
+                                              default-length-name))
+                        (,updater$a ,index
+                                    ,(cond
+                                       (element-copy
+                                        `(,element-copy ,initial-element ,element))
+                                       (element-fixer
+                                        `(,element-fixer ,element))
+                                       (t
+                                        `((lambda (x) x) ,element)))
+                                    (,copy ,%vector ,vector))
+                        (,copy ,%vector ,vector)))
+             :hints
+             (("Goal"
+               :by (:functional-instance
+                    ,(if resizable
+                         'lem-vector$a::copy/resizable-of-updater/resizable
+                         'lem-vector$a::copy/fixed-of-updater/fixed)
+                    ,@fi-bindings-with-copy)))))
+
+         (defthm ,copy-of-updater$a
+           (equal (,copy ,%vector (,updater$a ,index ,element ,vector))
+                  (if (< (nfix ,index) ,(if resizable
+                                            `(,length$a ,vector)
+                                            default-length-name))
+                      (,updater$a ,index
+                                  ,(if element-copy
+                                       `(,element-copy ,initial-element ,element)
+                                       element)
+                                  (,copy ,%vector ,vector))
+                      (,copy ,%vector ,vector)))
+           :hints
+           (("Goal"
+             :in-theory (enable ,vector$a-aggressive)
+             :use ,copy-of-updater$a-lemma)))
 
          (defthm ,copy-rw
            ,(if element-coupled-p
@@ -657,8 +795,19 @@
        (deflabel ,copy-end)
 
        (deftheory-static ,copy-theory
-         (set-difference-theories (current-theory ',copy-end)
-                                  (current-theory ',copy-begin))))))
+         (set-difference-theories
+          (set-difference-theories (current-theory ',copy-end)
+                                   (current-theory ',copy-begin))
+          '(,@(and element-coupled-p
+                   `(,coupledp
+                     ,coupledp-constraints))
+            ,copy-rec
+            ,copy
+            ,vector-copy-constraints)))
+
+       (in-theory
+         (union-theories (current-theory ',copy-begin)
+                         (theory ',copy-theory))))))
 
 
 ;;;; `MAKE-HASH-TABLE-COPY-EVENTS'
@@ -671,18 +820,19 @@
   (let* ((%hash-table (symbolicate package-witness "%" hash-table))
          (copy (symbolicate package-witness hash-table "-COPY"))
          (copy-rec (symbolicate package-witness copy "-REC"))
-         (copy-rw (symbolicate package-witness copy "-RW"))
 
          (coupledp (symbolicate package-witness hash-table "-COUPLED-P"))
          (coupled-keys-p (symbolicate package-witness hash-table "-COUPLED-KEYS-P"))
          (coupled-keys-p-witness (symbolicate package-witness coupled-keys-p "-WITNESS"))
+         (coupled-keys-p-necc (symbolicate package-witness coupled-keys-p "-NECC"))
          (coupled-vals-p (symbolicate package-witness hash-table "-COUPLED-VALS-P"))
          (coupled-vals-p-witness (symbolicate package-witness coupled-vals-p "-WITNESS"))
+         (coupled-vals-p-necc (symbolicate package-witness coupled-vals-p "-NECC"))
 
          ;; `HASH-TABLE'
          (stobj-property (getpropc hash-table 'acl2::stobj))
          (recognizer (caadr stobj-property))
-         (fixer (first (third stobj-property)))
+         (the-hash-table (symbolicate hash-table "THE-" hash-table))
          (accessor (second (third stobj-property)))
          (updater (third (third stobj-property)))
          (count (seventh (third stobj-property)))
@@ -694,12 +844,13 @@
          (world (w state))
          (stobj$a-property (cdr (assoc hash-table (table-alist 'stobj$a-property world))))
          (hash-table$a (first stobj$a-property))
-         (hash-table$a-definitions (symbolicate hash-table$a hash-table$a "-DEFINITIONS"))
          (hash-table$a-theorems (symbolicate hash-table$a hash-table$a "-THEOREMS"))
          (hash-table$a-aggressive (symbolicate hash-table$a hash-table$a "-AGGRESSIVE"))
+         (hash-table$a-constraints (symbolicate hash-table$a hash-table$a "-CONSTRAINTS"))
          (recognizer$a (first (second stobj$a-property)))
          (creator$a (second (second stobj$a-property)))
          (fixer$a (third (second stobj$a-property)))
+         (equiv$a (fourth (second stobj$a-property)))
          (accessor$a (first (fourth (third stobj$a-property))))
          (updater$a (second (fourth (third stobj$a-property))))
          (boundp$a (third (fourth (third stobj$a-property))))
@@ -708,10 +859,10 @@
          (count$a (sixth (fourth (third stobj$a-property))))
          (clear$a (seventh (fourth (third stobj$a-property))))
          (init$a (eighth (fourth (third stobj$a-property))))
-         (keysp$a (nth 8 (fourth (third stobj$a-property))))
-         (keys$a-fix (nth 9 (fourth (third stobj$a-property))))
-         (keys$a (nth 10 (fourth (third stobj$a-property))))
-         (keys-set$a (nth 11 (fourth (third stobj$a-property))))
+         (keys$a (first (fifth (third stobj$a-property))))
+         (keys$a-set (second (fifth (third stobj$a-property))))
+         (keys$ap (third (fifth (third stobj$a-property))))
+         (keys$a-fix (fourth (fifth (third stobj$a-property))))
 
          (contents$a (symbolicate hash-table$a hash-table$a "-CONTENTS"))
          (contents-recognizer$a (symbolicate hash-table$a contents$a "-P"))
@@ -719,19 +870,22 @@
          (contents-fixer$a (symbolicate hash-table$a contents$a "-FIX"))
          (contents-accessor$a (symbolicate hash-table$a contents$a "-GET"))
          (contents-updater$a (symbolicate hash-table$a contents$a "-PUT"))
-         (contents-boundp$a (symbolicate hash-table$a contents$a "-BOUNDP"))
+         (contents-boundp$a (symbolicate hash-table$a contents$a "-BNDP"))
          (contents-getp$a (symbolicate hash-table$a contents$a "-GETP"))
          (contents-remover$a (symbolicate hash-table$a contents$a "-REM"))
-         (contents-count$a (symbolicate hash-table$a contents$a "-COUNT"))
-         (contents-clear$a (symbolicate hash-table$a contents$a "-CLEAR"))
+         (contents-count$a (symbolicate hash-table$a contents$a "-CNT"))
+         (contents-clear$a (symbolicate hash-table$a contents$a "-CLR"))
          (contents-init$a (symbolicate hash-table$a contents$a "-INIT"))
 
          (key (first (first (third stobj$a-property))))
+         (%key (symbolicate key "%" key))
          (key-recognizer (second (first (third stobj$a-property))))
          (default-key-name (third (first (third stobj$a-property))))
          (key-fixer (fourth (first (third stobj$a-property))))
+         (key-equiv (fifth (first (third stobj$a-property))))
 
          (val (first (second (third stobj$a-property))))
+         (%val (symbolicate val "%" val))
          (val-stobj-property (getpropc val 'acl2::stobj))
          (val-stobj$a-property (cdr (assoc val (table-alist 'stobj$a-property world))))
          (val-recognizer (second (second (third stobj$a-property))))
@@ -741,11 +895,9 @@
                           `(,val-creator)
                           default-val-name))
          (val-fixer (fourth (second (third stobj$a-property))))
+         (val-equiv (fifth (second (third stobj$a-property))))
 
          ;; Adjust for nested stobj interface shuffle
-         (fixer (if val-stobj-property
-                    (third (third stobj-property))
-                    fixer))
          (accessor (if val-stobj-property
                        (first (third stobj-property))
                        accessor))
@@ -757,7 +909,6 @@
 
          (val-copy (cdr (assoc val (table-alist 'copy world))))
          (val-copy-theory (symbolicate val-copy val-copy "-THEORY"))
-         (%val (car (getpropc val-copy 'acl2::formals)))
          (val-coupled-p (cdr (assoc val (table-alist 'coupledp world))))
 
          (copy-begin (symbolicate package-witness copy "-BEGIN"))
@@ -765,115 +916,121 @@
          (copy-theory (symbolicate package-witness copy "-THEORY"))
 
          ;; Theorem Names
-         (booleanp-of-key-recognizer (symbolicate "ATOMIC-STOBJS" "BOOLEANP-OF-" key-recognizer))
-         (key-recognizer-of-default-key (symbolicate "ATOMIC-STOBJS" key-recognizer "-OF-DEFAULT-KEY"))
-         (key-fixer-rw (symbolicate "ATOMIC-STOBJS" key-fixer "-RW"))
+         (key-recognizer-constraints (symbolicate "ATOMIC-STOBJS" key-recognizer "-CONSTRAINTS"))
+         (key-fixer-constraints (symbolicate "ATOMIC-STOBJS" key-fixer "-CONSTRAINTS"))
+         (key-equiv-constraints (symbolicate "ATOMIC-STOBJS" key-equiv "-CONSTRAINTS"))
 
-         (booleanp-of-val-recognizer (symbolicate "ATOMIC-STOBJS" "BOOLEANP-OF-" val-recognizer))
-         (val-recognizer-of-default-val (symbolicate "ATOMIC-STOBJS" val-recognizer "-OF-DEFAULT-VAL"))
-         (val-fixer-rw (symbolicate "ATOMIC-STOBJS" val-fixer "-RW"))
+         (val-recognizer-constraints (symbolicate "ATOMIC-STOBJS" val-recognizer "-CONSTRAINTS"))
+         (val-fixer-constraints (symbolicate "ATOMIC-STOBJS" val-fixer "-CONSTRAINTS"))
+         (val-equiv-constraints (symbolicate "ATOMIC-STOBJS" val-equiv "-CONSTRAINTS"))
 
-         (coupled-keys-p-constraint-1 (symbolicate "ATOMIC-STOBJS" coupled-keys-p "-CONSTRAINT-1"))
-         (coupled-keys-p-constraint-2 (symbolicate "ATOMIC-STOBJS" coupled-keys-p "-CONSTRAINT-2"))
-         (coupled-vals-p-constraint-1 (symbolicate "ATOMIC-STOBJS" coupled-vals-p "-CONSTRAINT-1"))
-         (coupled-vals-p-constraint-2 (symbolicate "ATOMIC-STOBJS" coupled-vals-p "-CONSTRAINT-2"))
-         (coupled-keys-p-constraint-1/expanded (symbolicate "ATOMIC-STOBJS" coupled-keys-p-constraint-1 "/EXPANDED"))
-         (coupled-keys-p-constraint-2/expanded (symbolicate "ATOMIC-STOBJS" coupled-keys-p-constraint-2 "/EXPANDED"))
-         (coupled-vals-p-constraint-1/expanded (symbolicate "ATOMIC-STOBJS" coupled-vals-p-constraint-1 "/EXPANDED"))
-         (coupled-vals-p-constraint-2/expanded (symbolicate "ATOMIC-STOBJS" coupled-vals-p-constraint-2 "/EXPANDED"))
-         (coupledp/expanded (symbolicate "ATOMIC-STOBJS" coupledp "/EXPANDED"))
-         (copy-rec-of-fixer$a-3 (symbolicate "ATOMIC-STOBJS" copy-rec "-OF-" fixer$a "-3"))
-         (copy-rec-constraint (symbolicate "ATOMIC-STOBJS" copy-rec "-CONSTRAINT"))
-
+         (coupledp-constraints (symbolicate package-witness coupledp "-CONSTRAINTS"))
+         (coupledp-tp (symbolicate package-witness coupledp "-TP"))
          (coupledp-when-not-recognizer$a (symbolicate package-witness coupledp "-WHEN-NOT-" recognizer$a))
          (coupledp-of-creator$a (symbolicate package-witness coupledp "-OF-" creator$a))
-         (coupledp-of-fixer$a (symbolicate package-witness coupledp "-OF-" fixer$a))
+         (val-coupled-p-of-accessor$a (symbolicate package-witness val-coupled-p "-OF-" accessor$a))
          (coupledp-of-updater$a-when-boundp$a (symbolicate package-witness coupledp "-OF-" updater$a "-WHEN-" boundp$a))
-         (coupledp-of-updater$a-when-boundp$a-lemma (symbolicate package-witness coupledp-of-updater$a-when-boundp$a "-LEMMA"))
          (coupledp-of-updater$a-when-not-boundp$a (symbolicate package-witness coupledp "-OF-" updater$a "-WHEN-NOT-" boundp$a))
-         (coupledp-of-updater$a-when-not-boundp$a-lemma (symbolicate package-witness coupledp-of-updater$a-when-not-boundp$a "-LEMMA"))
+         (in-of-keys$a-when-coupledp (symbolicate package-witness "IN-OF-" keys$a "-WHEN-" coupledp))
          (coupledp-of-remover$a-when-boundp$a (symbolicate package-witness coupledp "-OF-" remover$a "-WHEN-" boundp$a))
          (coupledp-of-remover$a-when-not-boundp$a (symbolicate package-witness coupledp "-OF-" remover$a "-WHEN-NOT-" boundp$a))
          (cardinality-of-keys$a-when-coupledp (symbolicate package-witness "CARDINALITY-OF-" keys$a "-WHEN-" coupledp))
-         (in-of-keys$a-when-coupledp (symbolicate package-witness "IN-OF-" keys$a "-WHEN-" coupledp))
-         (val-coupled-p-of-accessor$a (symbolicate package-witness val-coupled-p "-OF-" accessor$a))
          (emptyp-of-keys$a-when-coupledp (symbolicate package-witness "EMPTYP-OF-" keys$a "-WHEN-" coupledp))
 
+         (copy-rec-of-updater$a-2 (symbolicate "ATOMIC-STOBJS" copy-rec "-OF-" updater$a "-2"))
+         (copy-rec-of-updater$a-3 (symbolicate "ATOMIC-STOBJS" copy-rec "-OF-" updater$a "-3"))
+         (copy-rec-of-fixer$a-3 (symbolicate "ATOMIC-STOBJS" copy-rec "-OF-" fixer$a "-3"))
+
+         (hash-table-copy-constraints (symbolicate package-witness copy "-CONSTRAINTS"))
          (recognizer$a-of-copy (symbolicate package-witness recognizer$a "-OF-" copy))
          (copy-ignores-1 (symbolicate package-witness copy "-IGNORES-1"))
-         (copy-of-fixer$a-2 (symbolicate package-witness copy "-OF-" fixer$a "-2"))
+         (coupledp-of-copy (symbolicate package-witness coupledp "-OF-" copy))
+         (accessor$a-of-copy (symbolicate package-witness accessor$a "-OF-" copy))
+         (accessor$a-of-copy-lemma (symbolicate "ATOMIC-STOBJS" accessor$a-of-copy "-LEMMA"))
+         (copy-of-updater$a (symbolicate package-witness copy "-OF-" updater$a))
+         (copy-of-updater$a-lemma (symbolicate "ATOMIC-STOBJS" copy-of-updater$a "-LEMMA"))
+         (boundp$a-of-copy (symbolicate package-witness boundp$a "-OF-" copy))
+         (copy-of-remover$a (symbolicate package-witness copy "-OF-" remover$a))
+         (count$a-of-copy (symbolicate package-witness count$a "-OF-" copy))
          (keys$a-of-copy (symbolicate package-witness keys$a "-OF-" copy))
+         (copy-rw (symbolicate package-witness copy "-RW"))
 
          (fi-bindings
-          (list `(lem-hash-table$a::val-coupled-p ,(or val-coupled-p
-                                                       '(lambda (val)
-                                                         t)))
-                `(lem-hash-table$a::coupled-keys-p ,coupled-keys-p)
-                `(lem-hash-table$a::coupled-keys-p-witness ,coupled-keys-p-witness)
-                `(lem-hash-table$a::coupled-vals-p ,(if val-coupled-p
-                                                        coupled-vals-p
-                                                        '(lambda (hash-table)
-                                                          t)))
-                `(lem-hash-table$a::coupled-vals-p-witness ,(if val-coupled-p
-                                                                coupled-vals-p-witness
-                                                                `(lambda (hash-table)
-                                                                   ,default-key-name)))
-                `(lem-hash-table$a::coupledp ,coupledp)
-
-                `(lem-hash-table$a::keysp ,(if key-recognizer
-                                               keysp$a
-                                               'set::setp))
-                `(lem-hash-table$a::keys-fix ,(if key-recognizer
-                                                  keys$a-fix
-                                                  'set::sfix))
-                `(lem-hash-table$a::key-recognizer ,(or key-recognizer
-                                                        '(lambda (key)
-                                                          t)))
-                `(lem-hash-table$a::default-key (lambda ()
-                                                  ,default-key-name))
-                `(lem-hash-table$a::key-fixer ,(or key-fixer
-                                                   '(lambda (key)
-                                                     key)))
-                `(lem-hash-table$a::val-recognizer ,(or val-recognizer
+          (append
+           (and val-coupled-p
+                (list `(lem-hash-table$a::coupled-vals-p-witness ,coupled-vals-p-witness)))
+           (list `(lem-hash-table$a::val-coupled-p ,(or val-coupled-p
                                                         '(lambda (val)
                                                           t)))
-                `(lem-hash-table$a::default-val ,(or val-creator
-                                                     `(lambda ()
-                                                        ,default-val-name)))
-                `(lem-hash-table$a::val-fixer ,(or val-fixer
-                                                   '(lambda (val)
-                                                     val)))
+                 `(lem-hash-table$a::coupled-keys-p ,coupled-keys-p)
+                 `(lem-hash-table$a::coupled-keys-p-witness ,coupled-keys-p-witness)
+                 `(lem-hash-table$a::coupled-vals-p ,(if val-coupled-p
+                                                         coupled-vals-p
+                                                         '(lambda (hash-table)
+                                                           t)))
+                 `(lem-hash-table$a::coupledp ,coupledp)
 
-                `(lem-hash-table$a::recognizer/unique ,contents-recognizer$a)
-                `(lem-hash-table$a::creator/unique ,contents-creator$a)
-                `(lem-hash-table$a::fixer/unique ,contents-fixer$a)
-                `(lem-hash-table$a::accessor/unique ,contents-accessor$a)
-                `(lem-hash-table$a::updater/unique ,contents-updater$a)
-                `(lem-hash-table$a::boundp/unique ,contents-boundp$a)
-                `(lem-hash-table$a::getp/unique ,contents-getp$a)
-                `(lem-hash-table$a::remover/unique ,contents-remover$a)
-                `(lem-hash-table$a::count/unique ,contents-count$a)
-                `(lem-hash-table$a::clear/unique ,contents-clear$a)
-                `(lem-hash-table$a::init/unique ,contents-init$a)
+                 `(lem-hash-table$a::key-recognizer ,(or key-recognizer
+                                                         '(lambda (key)
+                                                           t)))
+                 `(lem-hash-table$a::default-key (lambda ()
+                                                   ,default-key-name))
+                 `(lem-hash-table$a::key-fixer ,(or key-fixer
+                                                    '(lambda (key)
+                                                      key)))
+                 `(lem-hash-table$a::key-equiv ,(or key-equiv
+                                                    'equal))
 
-                `(lem-hash-table$a::recognizer/copyable ,recognizer$a)
-                `(lem-hash-table$a::creator/copyable ,creator$a)
-                `(lem-hash-table$a::fixer/copyable ,fixer$a)
-                `(lem-hash-table$a::accessor/copyable ,accessor$a)
-                `(lem-hash-table$a::updater/copyable ,updater$a)
-                `(lem-hash-table$a::boundp/copyable ,boundp$a)
-                `(lem-hash-table$a::getp/copyable ,getp$a)
-                `(lem-hash-table$a::remover/copyable ,remover$a)
-                `(lem-hash-table$a::count/copyable ,count$a)
-                `(lem-hash-table$a::clear/copyable ,clear$a)
-                `(lem-hash-table$a::init/copyable ,init$a)
-                `(lem-hash-table$a::keys ,keys$a)
-                `(lem-hash-table$a::keys-set ,keys-set$a)))
+                 `(lem-hash-table$a::val-recognizer ,(or val-recognizer
+                                                         '(lambda (val)
+                                                           t)))
+                 `(lem-hash-table$a::default-val ,(or val-creator
+                                                      `(lambda ()
+                                                         ,default-val-name)))
+                 `(lem-hash-table$a::val-fixer ,(or val-fixer
+                                                    '(lambda (val)
+                                                      val)))
+                 `(lem-hash-table$a::val-equiv ,(or val-equiv
+                                                    'equal))
+
+                 `(lem-hash-table$a::keysp ,keys$ap)
+                 `(lem-hash-table$a::keys-fix ,keys$a-fix)
+                 `(lem-hash-table$a::recognizer/unique ,contents-recognizer$a)
+                 `(lem-hash-table$a::creator/unique ,contents-creator$a)
+                 `(lem-hash-table$a::fixer/unique ,contents-fixer$a)
+                 `(lem-hash-table$a::accessor/unique ,contents-accessor$a)
+                 `(lem-hash-table$a::updater/unique ,contents-updater$a)
+                 `(lem-hash-table$a::boundp/unique ,contents-boundp$a)
+                 `(lem-hash-table$a::getp/unique ,contents-getp$a)
+                 `(lem-hash-table$a::remover/unique ,contents-remover$a)
+                 `(lem-hash-table$a::count/unique ,contents-count$a)
+                 `(lem-hash-table$a::clear/unique ,contents-clear$a)
+                 `(lem-hash-table$a::init/unique ,contents-init$a)
+
+                 `(lem-hash-table$a::recognizer/copyable ,recognizer$a)
+                 `(lem-hash-table$a::creator/copyable ,creator$a)
+                 `(lem-hash-table$a::fixer/copyable ,fixer$a)
+                 `(lem-hash-table$a::equiv/copyable ,equiv$a)
+                 `(lem-hash-table$a::accessor/copyable ,accessor$a)
+                 `(lem-hash-table$a::updater/copyable ,updater$a)
+                 `(lem-hash-table$a::boundp/copyable ,boundp$a)
+                 `(lem-hash-table$a::getp/copyable ,getp$a)
+                 `(lem-hash-table$a::remover/copyable ,remover$a)
+                 `(lem-hash-table$a::count/copyable ,count$a)
+                 `(lem-hash-table$a::clear/copyable ,clear$a)
+                 `(lem-hash-table$a::init/copyable ,init$a)
+                 `(lem-hash-table$a::keys ,keys$a)
+                 `(lem-hash-table$a::keys-set ,keys$a-set))))
 
          (fi-bindings-with-copy
-          (list* `(lem-hash-table$a::val-copy ,(or val-copy
-                                                   `(lambda (%val val)
-                                                      (,val-fixer val))))
+          (list* `(lem-hash-table$a::val-copy ,(cond
+                                                 (val-copy)
+                                                 (val-fixer
+                                                  `(lambda (%val val)
+                                                     (,val-fixer val)))
+                                                 (t
+                                                  `(lambda (%val val)
+                                                     val))))
                  `(lem-hash-table$a::copy-rec ,copy-rec)
                  `(lem-hash-table$a::copy ,copy)
                  fi-bindings)))
@@ -886,47 +1043,56 @@
          (local
            (deflabel prologue-begin))
 
-         ,@(and key-recognizer
-                key-fixer
+         ,@(and key-fixer
+                key-recognizer
+                (not (eq key-equiv 'equal))
                 `((local
-                    (defthm ,booleanp-of-key-recognizer
-                      (booleanp (,key-recognizer ,key))
+                    (defthm ,key-recognizer-constraints
+                      (and (booleanp (,key-recognizer ,key))
+                           (,key-recognizer ,default-key-name))
                       :rule-classes
-                      (:rewrite
-                       :type-prescription)))
+                      ((:rewrite :corollary
+                                 (booleanp (,key-recognizer ,key))))))
 
                   (local
-                    (defthm ,key-recognizer-of-default-key
-                      (,key-recognizer ,default-key-name)
-                      :rule-classes nil))
-
-                  (local
-                    (defthm ,key-fixer-rw
+                    (defthm ,key-fixer-constraints
                       (equal (,key-fixer ,key)
                              (if (,key-recognizer ,key)
                                  ,key
-                                 ,default-key-name))))))
+                                 ,default-key-name))))
 
-         ,@(and val-recognizer
-                val-fixer
+                  (local
+                    (defthm ,key-equiv-constraints
+                      (equal (,key-equiv ,%key ,key)
+                             (equal (,key-fixer ,%key)
+                                    (,key-fixer ,key)))))))
+
+         ,@(and val-fixer
+                val-recognizer
+                (not (eq val-equiv 'equal))
                 `((local
-                    (defthm ,booleanp-of-val-recognizer
-                      (booleanp (,val-recognizer ,val))
+                    (defthm ,val-recognizer-constraints
+                      (and (booleanp (,val-recognizer ,val))
+                           (,val-recognizer ,default-val))
                       :rule-classes
-                      (:rewrite
-                       :type-prescription)))
+                      ((:rewrite :corollary
+                                 (booleanp (,val-recognizer ,val)))
+                       ,@(and (not (equal default-val default-val-name))
+                              `((:rewrite :corollary
+                                          (,val-recognizer ,default-val)))))))
 
                   (local
-                    (defthm ,val-recognizer-of-default-val
-                      (,val-recognizer ,default-val)
-                      :rule-classes nil))
-
-                  (local
-                    (defthm ,val-fixer-rw
+                    (defthm ,val-fixer-constraints
                       (equal (,val-fixer ,val)
                              (if (,val-recognizer ,val)
                                  ,val
-                                 ,default-val))))))
+                                 ,default-val))))
+
+                  (local
+                    (defthm ,val-equiv-constraints
+                      (equal (,val-equiv ,%val ,val)
+                             (equal (,val-fixer ,%val)
+                                    (,val-fixer ,val)))))))
 
          (local
            (deflabel prologue-end))
@@ -940,38 +1106,34 @@
          (local
            (in-theory
              (union-theories
-              (union-theories (theory 'acl2::ground-zero)
-                              (theory ',hash-table$a-definitions))
+              (theory 'acl2::ground-zero)
               (set-difference-theories (current-theory 'prologue-end)
                                        (current-theory 'prologue-begin)))))
 
-         ,@(and key-recognizer
-                key-fixer
-                `((local
-                    (in-theory
-                      (e/d ((:e ,key-recognizer)
-                            (:e ,key-fixer))
-                           (,key-recognizer
-                            ,key-fixer))))))
-
-         ,@(and val-recognizer
-                val-fixer
-                `((local
-                    (in-theory
-                      (e/d ((:e ,val-recognizer)
-                            (:e ,val-fixer))
-                           (,val-recognizer
-                            ,val-fixer))))))
-
-         ,@(and val-stobj$a-property
-                `((local
-                    (in-theory
-                      (disable ,val-creator)))))
-
-         ,@(and val-stobj-property
+         ,@(and val-copy
                 `((local
                     (in-theory
                       (enable ,val-copy-theory)))))
+
+         (local
+           (in-theory
+             (enable (:e set::emptyp)
+                     set::setp-type
+                     set::sets-are-true-lists-compound-recognizer
+                     set::tail-produces-set
+                     set::never-in-empty
+                     set::subset-reflexive
+                     set::head-unique)))
+
+         ,@(and key-recognizer
+                `((local
+                    (in-theory
+                      (enable (:e ,key-recognizer))))))
+
+         ,@(and val-recognizer
+                `((local
+                    (in-theory
+                      (enable (:e ,val-recognizer))))))
 
          ,@(and val-stobj-property
                 `((local
@@ -986,10 +1148,6 @@
            :package-witness ,package-witness
            :debug ,debug)
 
-         (local
-           (in-theory
-             (enable ,@(strip-cars (cdr (getpropc %hash-table 'acl2::absstobj-info))))))
-
          ;; `COUPLED-KEYS-P'
          (defun-sk ,coupled-keys-p (,hash-table)
            (declare (xargs :guard (,recognizer ,hash-table)
@@ -1002,35 +1160,6 @@
                          `(,boundp$a ,key ,hash-table))))
            :rewrite :direct)
 
-         (local
-           (defthmd ,coupled-keys-p-constraint-1
-             (implies (,coupled-keys-p ,hash-table)
-                      (equal (set::in ,key (,keys$a ,hash-table))
-                             ,(if key-recognizer
-                                  `(if (,key-recognizer ,key)
-                                       (,boundp$a ,key ,hash-table)
-                                       nil)
-                                  `(,boundp$a ,key ,hash-table))))
-             :hints
-             (("Goal"
-               :in-theory (disable ,coupled-keys-p
-                                   ,hash-table$a-definitions)))))
-
-         (local
-           (defthmd ,coupled-keys-p-constraint-2
-             (equal (,coupled-keys-p ,hash-table)
-                    ((lambda (,key ,hash-table)
-                       (equal (set::in ,key (,keys$a ,hash-table))
-                              ,(if key-recognizer
-                                   `(if (,key-recognizer ,key)
-                                        (,boundp$a ,key ,hash-table)
-                                        nil)
-                                   `(,boundp$a ,key ,hash-table))))
-                     (,coupled-keys-p-witness ,hash-table) ,hash-table))))
-
-         (in-theory
-           (disable ,coupled-keys-p))
-
          ;; `COUPLED-VALS-P'
          ,@(and val-coupled-p
                 `((defun-sk ,coupled-vals-p (,hash-table)
@@ -1038,26 +1167,7 @@
                                     :verify-guards nil))
                     (forall ,key
                       (,val-coupled-p (,accessor$a ,key ,hash-table)))
-                    :rewrite :direct)
-
-                  (local
-                    (defthmd ,coupled-vals-p-constraint-1
-                      (implies (,coupled-vals-p ,hash-table)
-                               (,val-coupled-p (,accessor$a ,key ,hash-table)))
-                      :hints
-                      (("Goal"
-                        :in-theory (disable ,coupled-vals-p
-                                            ,hash-table$a-definitions)))))
-
-                  (local
-                    (defthmd ,coupled-vals-p-constraint-2
-                      (equal (,coupled-vals-p ,hash-table)
-                             ((lambda (,key ,hash-table)
-                                (,val-coupled-p (,accessor$a ,key ,hash-table)))
-                              (,coupled-vals-p-witness ,hash-table) ,hash-table))))
-
-                  (in-theory
-                    (disable ,coupled-vals-p))))
+                    :rewrite :direct)))
 
          ;; `COUPLEDP'
          (defun-nx ,coupledp (,hash-table)
@@ -1071,85 +1181,139 @@
 
          (table coupledp ',hash-table ',coupledp)
 
-         (local
-           (defthmd ,coupled-keys-p-constraint-1/expanded
-             (implies (,coupled-keys-p ,hash-table)
-                      (equal (set::in ,key (car (,fixer$a ,hash-table)))
-                             ,(if key-recognizer
-                                  `(and (,key-recognizer ,key)
-                                        (,contents-boundp$a (,key-fixer ,key) (cdr (,fixer$a ,hash-table))))
-                                  `(,contents-boundp$a ,key (cdr (,fixer$a ,hash-table))))))
-             :hints
-             (("Goal"
-               :in-theory (disable ,hash-table$a-definitions)
-               :use ,coupled-keys-p-constraint-1
-               :expand ((:free (,key ,hash-table)
-                               (,boundp$a ,key ,hash-table))
-                        (:free (,hash-table)
-                               (,keys$a ,hash-table)))))))
+         (defthm ,coupledp-constraints
+           (and (equal (,coupled-keys-p ,hash-table)
+                       ((lambda (,key ,hash-table)
+                          (equal (set::in ,key (,keys$a ,hash-table))
+                                 ,(if key-recognizer
+                                      `(if (,key-recognizer ,key)
+                                           (,boundp$a ,key ,hash-table)
+                                           'nil)
+                                      `(,boundp$a ,key ,hash-table))))
+                        (,coupled-keys-p-witness ,hash-table)
+                        ,hash-table))
+                (implies (,coupled-keys-p ,hash-table)
+                         (equal (set::in ,key (,keys$a ,hash-table))
+                                ,(if key-recognizer
+                                     `(if (,key-recognizer ,key)
+                                          (,boundp$a ,key ,hash-table)
+                                          'nil)
+                                     `(,boundp$a ,key ,hash-table))))
+                ,@(and val-coupled-p
+                       `((equal (,coupled-vals-p ,hash-table)
+                                ((lambda (,key ,hash-table)
+                                   (,val-coupled-p (,accessor$a ,key ,hash-table)))
+                                 (,coupled-vals-p-witness ,hash-table)
+                                 ,hash-table))
+                         (implies (,coupled-vals-p ,hash-table)
+                                  (,val-coupled-p (,accessor$a ,key ,hash-table)))))
+                (equal (,coupledp ,hash-table)
+                       (if (equal (set::cardinality (,keys$a ,hash-table))
+                                  (,count$a ,hash-table))
+                           ,(if val-coupled-p
+                                `(if (,coupled-keys-p ,hash-table)
+                                     (,coupled-vals-p ,hash-table)
+                                     'nil)
+                                `(,coupled-keys-p ,hash-table))
+                           'nil)))
+           :rule-classes
+           ((:definition :corollary
+                (equal (,coupled-keys-p ,hash-table)
+                       ((lambda (,key ,hash-table)
+                          (equal (set::in ,key (,keys$a ,hash-table))
+                                 ,(if key-recognizer
+                                      `(if (,key-recognizer ,key)
+                                           (,boundp$a ,key ,hash-table)
+                                           'nil)
+                                      `(,boundp$a ,key ,hash-table))))
+                        (,coupled-keys-p-witness ,hash-table)
+                        ,hash-table)))
+            (:rewrite :corollary
+                      (implies (,coupled-keys-p ,hash-table)
+                               (equal (set::in ,key (,keys$a ,hash-table))
+                                      ,(if key-recognizer
+                                           `(if (,key-recognizer ,key)
+                                                (,boundp$a ,key ,hash-table)
+                                                'nil)
+                                           `(,boundp$a ,key ,hash-table)))))
+            ,@(and val-coupled-p
+                   `((:definition :corollary
+                         (equal (,coupled-vals-p ,hash-table)
+                                ((lambda (,key ,hash-table)
+                                   (,val-coupled-p (,accessor$a ,key ,hash-table)))
+                                 (,coupled-vals-p-witness ,hash-table)
+                                 ,hash-table)))
+                     (:rewrite :corollary
+                               (implies (,coupled-vals-p ,hash-table)
+                                        (,val-coupled-p (,accessor$a ,key ,hash-table))))))
+            (:definition :corollary
+                (equal (,coupledp ,hash-table)
+                       (if (equal (set::cardinality (,keys$a ,hash-table))
+                                  (,count$a ,hash-table))
+                           ,(if val-coupled-p
+                                `(if (,coupled-keys-p ,hash-table)
+                                     (,coupled-vals-p ,hash-table)
+                                     'nil)
+                                `(,coupled-keys-p ,hash-table))
+                           'nil))))
+           :hints
+           (("Goal"
+             :in-theory (disable ,coupled-keys-p-necc
+                                 ,@(and val-coupled-p
+                                        `(,coupled-vals-p-necc)))
+             :use ((:instance ,coupled-keys-p-necc)
+                   ,@(and val-coupled-p
+                          `((:instance ,coupled-vals-p-necc)))))))
 
          (local
-           (defthmd ,coupled-keys-p-constraint-2/expanded
-             (equal (,coupled-keys-p ,hash-table)
-                    (let ((,key (,coupled-keys-p-witness ,hash-table)))
-                      (equal (set::in ,key (car (,fixer$a ,hash-table)))
-                             ,(if key-recognizer
-                                  `(and (,key-recognizer ,key)
-                                        (,contents-boundp$a (,key-fixer ,key) (cdr (,fixer$a ,hash-table))))
-                                  `(,contents-boundp$a ,key (cdr (,fixer$a ,hash-table)))))))
-             :hints
-             (("Goal"
-               :in-theory (disable ,hash-table$a-definitions)
-               :use ,coupled-keys-p-constraint-2
-               :expand ((:free (,key ,hash-table)
-                               (,boundp$a ,key ,hash-table))
-                        (:free (,hash-table)
-                               (,keys$a ,hash-table)))))))
+           (in-theory
+             (disable ,coupledp
+                      ,coupled-keys-p
+                      (:definition ,coupledp-constraints . 1)
+                      ,@(and val-coupled-p
+                             `(,coupled-vals-p
+                               (:definition ,coupledp-constraints . 2))))))
 
-         ,@(and val-coupled-p
-                `((local
-                    (defthmd ,coupled-vals-p-constraint-1/expanded
-                      (implies (,coupled-vals-p ,hash-table)
-                               (,val-coupled-p (,contents-accessor$a ,(if key-fixer
-                                                                          `(,key-fixer ,key)
-                                                                          key)
-                                                                     (cdr (,fixer$a ,hash-table)))))
-                      :hints
-                      (("Goal"
-                        :in-theory (disable ,hash-table$a-definitions)
-                        :use ,coupled-vals-p-constraint-1
-                        :expand ((:free (,key ,hash-table)
-                                        (,accessor$a ,key ,hash-table)))))))
-
-                  (local
-                    (defthmd ,coupled-vals-p-constraint-2/expanded
-                      (equal (,coupled-vals-p ,hash-table)
-                             (,val-coupled-p (,contents-accessor$a ,(if key-fixer
-                                                                        `(,key-fixer (,coupled-vals-p-witness ,hash-table))
-                                                                        `(,coupled-vals-p-witness ,hash-table))
-                                                                   (cdr (,fixer$a ,hash-table)))))
-                      :hints
-                      (("Goal"
-                        :in-theory (disable ,hash-table$a-definitions)
-                        :use ,coupled-vals-p-constraint-2
-                        :expand ((:free (,key ,hash-table)
-                                        (,accessor$a ,key ,hash-table)))))))))
-
-         (local
-           (defthmd ,coupledp/expanded
-             (equal (,coupledp ,hash-table)
-                    (and (equal (set::cardinality (car (,fixer$a ,hash-table)))
-                                (,contents-count$a (cdr (,fixer$a ,hash-table))))
-                         (,coupled-keys-p ,hash-table)
-                         ,@(and val-coupled-p
-                                `((,coupled-vals-p ,hash-table)))))
-             :hints
-             (("Goal"
-               :in-theory (disable ,hash-table$a-definitions)
-               :expand ((:free (,hash-table)
-                               (,keys$a ,hash-table))
-                        (:free (,hash-table)
-                               (,count$a ,hash-table)))))))
+         (defthm ,coupledp-tp
+           (booleanp (,coupledp ,hash-table))
+           :rule-classes :type-prescription
+           :hints
+           (("Goal"
+             :in-theory (enable ,hash-table$a-constraints)
+             :by (:functional-instance
+                  lem-hash-table$a::coupledp-tp
+                  ,@fi-bindings))
+            ,@(and val-coupled-p
+                   key-recognizer
+                   `(("Subgoal 14"
+                      :in-theory (e/d (,hash-table$a-constraints)
+                                      (,coupled-vals-p-necc))
+                      :use ((:instance ,coupled-vals-p-necc
+                                       (,hash-table lem-hash-table$a::hash-table)
+                                       (,key lem-hash-table$a::key))))
+                     ("Subgoal 13"
+                      :use ((:instance (:definition ,coupledp-constraints . 2)
+                                       (,hash-table lem-hash-table$a::hash-table))))))
+            ,@(and val-coupled-p
+                   (not key-recognizer)
+                   `(("Subgoal 13"
+                      :in-theory (e/d (,hash-table$a-constraints)
+                                      (,coupled-vals-p-necc))
+                      :use ((:instance ,coupled-vals-p-necc
+                                       (,hash-table lem-hash-table$a::hash-table)
+                                       (,key lem-hash-table$a::key))))
+                     ("Subgoal 12"
+                      :use ((:instance (:definition ,coupledp-constraints . 2)
+                                       (,hash-table lem-hash-table$a::hash-table))))))
+            ("Subgoal 4"
+             :in-theory (e/d (,hash-table$a-constraints)
+                             (,coupled-keys-p-necc))
+             :use ((:instance ,coupled-keys-p-necc
+                              (,hash-table lem-hash-table$a::hash-table)
+                              (,key lem-hash-table$a::key))))
+            ("Subgoal 3"
+             :use ((:instance (:definition ,coupledp-constraints . 1)
+                              (,hash-table lem-hash-table$a::hash-table))))))
 
          (defthm ,coupledp-when-not-recognizer$a
            (implies (not (,recognizer$a ,hash-table))
@@ -1157,49 +1321,9 @@
            :hints
            (("Goal"
              :do-not-induct t
-             :in-theory (enable set::in
-                                set::emptyp
-                                set::setp)
              :by (:functional-instance
                   lem-hash-table$a::coupledp-when-not-recognizer/copyable
-                  ,@fi-bindings))
-            ,@(and val-coupled-p
-                   `(,@(if key-recognizer
-                           `(("Subgoal 14"
-                              :in-theory (theory 'acl2::minimal-theory)
-                              :use (:instance ,coupled-vals-p-constraint-1/expanded
-                                              (,key lem-hash-table$a::key)
-                                              (,hash-table acl2::hash-table)))
-                             ("Subgoal 13"
-                              :in-theory (theory 'acl2::minimal-theory)
-                              :use (:instance ,coupled-vals-p-constraint-2/expanded
-                                              (,hash-table acl2::hash-table))))
-                           `(("Subgoal 14"
-                              :in-theory (theory 'acl2::minimal-theory)
-                              :use (:instance ,coupledp/expanded
-                                              (,hash-table acl2::hash-table)))
-                             ("Subgoal 13"
-                              :in-theory (theory 'acl2::minimal-theory)
-                              :use (:instance ,coupled-vals-p-constraint-1/expanded
-                                              (,key lem-hash-table$a::key)
-                                              (,hash-table acl2::hash-table)))
-                             ("Subgoal 12"
-                              :in-theory (theory 'acl2::minimal-theory)
-                              :use (:instance ,coupled-vals-p-constraint-2/expanded
-                                              (,hash-table acl2::hash-table)))))))
-            ,@(and (not key-recognizer)
-                   `(("Subgoal 7"
-                      :in-theory (enable set::setp
-                                         acl2::fast-<<-is-<<))))
-            ("Subgoal 4"
-             :in-theory (theory 'acl2::minimal-theory)
-             :use (:instance ,coupled-keys-p-constraint-1/expanded
-                             (,key lem-hash-table$a::key)
-                             (,hash-table acl2::hash-table)))
-            ("Subgoal 3"
-             :in-theory (theory 'acl2::minimal-theory)
-             :use (:instance ,coupled-keys-p-constraint-2/expanded
-                             (,hash-table acl2::hash-table)))))
+                  ,@fi-bindings))))
 
          (defthm ,coupledp-of-creator$a
            (,coupledp (,creator$a))
@@ -1209,95 +1333,56 @@
                   lem-hash-table$a::coupledp-of-creator/copyable
                   ,@fi-bindings))))
 
-         (defthm ,coupledp-of-fixer$a
-           (equal (,coupledp (,fixer$a ,hash-table))
-                  (,coupledp ,hash-table))
+         (defcong ,equiv$a equal (,coupledp ,hash-table) 1
            :hints
            (("Goal"
+             :in-theory (enable ,equiv$a)
              :by (:functional-instance
-                  lem-hash-table$a::coupledp-of-fixer/copyable
+                  lem-hash-table$a::equiv/copyable-implies-equal-coupledp-1
                   ,@fi-bindings))))
 
          ,@(and val-coupled-p
                 `((defthm ,val-coupled-p-of-accessor$a
                     (implies (,coupledp ,hash-table)
                              (,val-coupled-p (,accessor$a ,key ,hash-table)))
-                    :rule-classes
-                    ((:rewrite :corollary
-                               (implies (coupledp ,hash-table)
-                                        (,val-coupled-p (,accessor$a ,key ,hash-table)))))
                     :hints
                     (("Goal"
                       :by (:functional-instance
                            lem-hash-table$a::val-coupled-p-of-accessor/copyable
                            ,@fi-bindings))))))
 
-         ,@(and (not val-coupled-p)
-                `((local
-                    (defthm ,coupledp-of-updater$a-when-boundp$a-lemma
-                      (implies (and (,boundp$a ,key ,hash-table)
-                                    (,coupledp ,hash-table))
-                               (equal (,coupledp (,updater$a ,key ,val ,hash-table))
-                                      t))
-                      :hints
-                      (("Goal"
-                        :do-not-induct t
-                        :by (:functional-instance
-                             lem-hash-table$a::coupledp-of-updater/copyable-when-boundp/copyable
-                             ,@fi-bindings)))))))
-
          (defthm ,coupledp-of-updater$a-when-boundp$a
            (implies (and (,boundp$a ,key ,hash-table)
                          (,coupledp ,hash-table))
-                    ,(if val-coupled-p
-                         `(equal (,coupledp (,updater$a ,key ,val ,hash-table))
-                                 (,val-coupled-p ,val))
-                         `(,coupledp (,updater$a ,key ,val ,hash-table))))
+                    (equal (,coupledp (,updater$a ,key ,val ,hash-table))
+                           ,(if val-coupled-p
+                                `(,val-coupled-p ,val)
+                                't)))
            :hints
            (("Goal"
              :do-not-induct t
-             ,@(if val-coupled-p
-                   `(:by (:functional-instance
-                          lem-hash-table$a::coupledp-of-updater/copyable-when-boundp/copyable
-                          ,@fi-bindings))
-                   `(:use ,coupledp-of-updater$a-when-boundp$a-lemma)))))
-
-         ,@(and (not val-coupled-p)
-                `((defthm ,coupledp-of-updater$a-when-not-boundp$a-lemma
-                    (implies (let* ((,keys$a (,keys$a ,hash-table))
-                                    (trimmed (set::delete ,(if key-fixer `(,key-fixer ,key) key) ,keys$a)))
-                               (and (not (,boundp$a ,key ,hash-table))
-                                    (set::in ,(if key-fixer `(,key-fixer ,key) key) ,keys$a)
-                                    (,coupledp (,keys-set$a trimmed ,hash-table))))
-                             (equal (,coupledp (,updater$a ,key ,val ,hash-table))
-                                    t))
-                    :hints
-                    (("Goal"
-                      :do-not-induct t
-                      :in-theory (enable set::sfix-set-identity)
-                      :by (:functional-instance
-                           lem-hash-table$a::coupledp-of-updater/copyable-when-not-boundp/copyable
-                           ,@fi-bindings))))))
+             :in-theory (enable ,hash-table$a-constraints)
+             :by (:functional-instance
+                  lem-hash-table$a::coupledp-of-updater/copyable-when-boundp/copyable
+                  ,@fi-bindings))))
 
          (defthm ,coupledp-of-updater$a-when-not-boundp$a
            (implies (let* ((,keys$a (,keys$a ,hash-table))
                            (trimmed (set::delete ,(if key-fixer `(,key-fixer ,key) key) ,keys$a)))
                       (and (not (,boundp$a ,key ,hash-table))
                            (set::in ,(if key-fixer `(,key-fixer ,key) key) ,keys$a)
-                           (,coupledp (,keys-set$a trimmed ,hash-table))))
-                    ,(if val-coupled-p
-                         `(equal (,coupledp (,updater$a ,key ,val ,hash-table))
-                                 (,val-coupled-p ,val))
-                         `(,coupledp (,updater$a ,key ,val ,hash-table))))
+                           (,coupledp (,keys$a-set trimmed ,hash-table))))
+                    (equal (,coupledp (,updater$a ,key ,val ,hash-table))
+                           ,(if val-coupled-p
+                                `(,val-coupled-p ,val)
+                                't)))
            :hints
            (("Goal"
              :do-not-induct t
-             :in-theory (enable set::sfix-set-identity)
-             ,@(if val-coupled-p
-                   `(:by (:functional-instance
-                          lem-hash-table$a::coupledp-of-updater/copyable-when-not-boundp/copyable
-                          ,@fi-bindings))
-                   `(:use ,coupledp-of-updater$a-when-not-boundp$a-lemma)))))
+             :in-theory (enable ,hash-table$a-constraints)
+             :by (:functional-instance
+                  lem-hash-table$a::coupledp-of-updater/copyable-when-not-boundp/copyable
+                  ,@fi-bindings))))
 
          (defthm ,in-of-keys$a-when-coupledp
            (implies (,coupledp ,hash-table)
@@ -1306,6 +1391,14 @@
                                 `(and (,key-recognizer ,key)
                                       (,boundp$a ,key ,hash-table))
                                 `(,boundp$a ,key ,hash-table))))
+           :rule-classes
+           ((:rewrite :corollary
+                      (implies (,coupledp ,hash-table)
+                               (equal (set::in ,key (,keys$a ,hash-table))
+                                      ,(if key-recognizer
+                                           `(and (,key-recognizer ,key)
+                                                 (,boundp$a (double-rewrite ,key) ,hash-table))
+                                           `(,boundp$a (double-rewrite ,key) ,hash-table))))))
            :hints
            (("Goal"
              :by (:functional-instance
@@ -1317,11 +1410,12 @@
                            (inserted (set::insert ,(if key-fixer `(,key-fixer ,key) key) ,keys$a)))
                       (and (,boundp$a ,key ,hash-table)
                            (not (set::in ,(if key-fixer `(,key-fixer ,key) key) ,keys$a))
-                           (,coupledp (,keys-set$a inserted ,hash-table))))
+                           (,coupledp (,keys$a-set inserted ,hash-table))))
                     (,coupledp (,remover$a ,key ,hash-table)))
            :hints
            (("Goal"
              :do-not-induct t
+             :in-theory (enable ,hash-table$a-constraints)
              :by (:functional-instance
                   lem-hash-table$a::coupledp-of-remover/copyable-when-boundp/copyable
                   ,@fi-bindings))))
@@ -1349,38 +1443,33 @@
          (defthm ,emptyp-of-keys$a-when-coupledp
            (implies (,coupledp ,hash-table)
                     (equal (set::emptyp (,keys$a ,hash-table))
-                           (or (not (,recognizer$a ,hash-table))
-                               (equal ,hash-table (,creator$a)))))
+                           (,equiv$a ,hash-table (,creator$a))))
            :hints
            (("Goal"
              :by (:functional-instance
                   lem-hash-table$a::emptyp-of-keys-when-coupledp
                   ,@fi-bindings))))
 
-         (in-theory
-           (disable ,coupledp))
-
          ;; `COPY-REC'
          (defun ,copy-rec (set ,%hash-table ,hash-table)
            (declare (xargs :stobjs (,%hash-table ,hash-table)
-                           :guard (and (,keysp$a set)
+                           :guard (and (,keys$ap set)
                                        (set::subset set (,keys ,hash-table)))
                            :guard-hints
                            (("Goal"
-                             :in-theory (e/d (set::subset
-                                              set::emptyp
-                                              set::setp
-                                              ,hash-table$a-theorems
-                                              ,hash-table$a-aggressive)
-                                             (,hash-table$a-definitions))))
+                             :in-theory (enable ,hash-table$a-theorems
+                                                ,hash-table$a-aggressive
+                                                set::subset
+                                                set::emptyp
+                                                set::in)))
                            :measure (set::cardinality set)
                            :hints
                            (("Goal"
                              :in-theory (enable set::cardinality)))))
            (if (mbe :logic (or (set::emptyp set)
-                               (not (,keysp$a set)))
+                               (not (,keys$ap set)))
                     :exec (endp set))
-               (,fixer ,%hash-table)
+               (,the-hash-table ,%hash-table)
                ,(if val-copy
                     `(let ((,key (set::head set)))
                        (stobj-let ((,val (,accessor ,key ,hash-table) ,updater))
@@ -1395,69 +1484,13 @@
                             (,%hash-table (,updater ,key ,val ,%hash-table)))
                        (,copy-rec (set::tail set) ,%hash-table ,hash-table)))))
 
-         (local
-           (defthm ,copy-rec-of-fixer$a-3
-             (equal (,copy-rec set ,%hash-table (,fixer$a ,hash-table))
-                    (,copy-rec set ,%hash-table ,hash-table))
-             :hints
-             (("Goal"
-               :in-theory (e/d (,hash-table$a-theorems
-                                ,hash-table$a-aggressive)
-                               (,hash-table$a-definitions))))))
-
-         (local
-           (defthm copy-rec-of-updater$a-when-not-in
-             (implies (and (,keysp$a set)
-                           (not (set::in ,(if key-fixer
-                                              `(,key-fixer ,key)
-                                              key)
-                                         set)))
-                      (equal (,copy-rec set ,%hash-table (,updater$a ,key ,val ,hash-table))
-                             (,copy-rec set ,%hash-table ,hash-table)))
-             :hints
-             (("Goal"
-               :in-theory (e/d (,hash-table$a-theorems
-                                ,hash-table$a-aggressive
-                                set::in)
-                               (,hash-table$a-definitions))))))
-
-         (local
-           (defthm ,copy-rec-constraint
-             (equal (,copy-rec set ,%hash-table ,hash-table)
-                    (if (or (set::emptyp set)
-                            (not (,keysp$a set)))
-                        (,fixer$a ,%hash-table)
-                        (let* ((,key (set::head set))
-                               (val (,accessor$a ,key ,hash-table))
-                               (%val (,accessor$a ,key ,%hash-table)))
-                          (declare (ignorable %val))
-                          (let* ((%val ,(if val-copy
-                                            `(,val-copy %val val)
-                                            `(,val-fixer val)))
-                                 (,%hash-table (,updater$a ,key %val ,%hash-table))
-                                 (,hash-table (,updater$a ,key val ,hash-table)))
-                            (,copy-rec (set::tail set) ,%hash-table ,hash-table)))))
-             :hints
-             (("Goal"
-               :do-not-induct t
-               :in-theory (e/d (,hash-table$a-theorems
-                                ,hash-table$a-aggressive
-                                set::head-unique
-                                set::tail-produces-set)
-                               (,hash-table$a-definitions))))))
-
-         (in-theory
-           (disable ,copy-rec))
-
          ;; `COPY'
          (defun ,copy (,%hash-table ,hash-table)
            (declare (xargs :stobjs (,%hash-table ,hash-table)
                            :guard-hints
                            (("Goal"
-                             :in-theory (e/d (set::subset-reflexive
-                                              ,hash-table$a-theorems
-                                              ,hash-table$a-aggressive)
-                                             (,hash-table$a-definitions))))))
+                             :in-theory (enable ,hash-table$a-theorems
+                                                ,hash-table$a-aggressive)))))
            (let* ((,keys (,keys ,hash-table))
                   (,count (,count ,hash-table))
                   (,%hash-table (,init ,count nil nil ,%hash-table))
@@ -1466,14 +1499,175 @@
 
          (table copy ',hash-table ',copy)
 
+         (local
+           (defthmd ,copy-rec-of-updater$a-2
+             (implies (,keys$ap set)
+                      (equal (,copy-rec set (,updater$a ,key ,val ,%hash-table) ,hash-table)
+                             (if (set::in ,(if key-fixer `(,key-fixer ,key) key) set)
+                                 (,copy-rec set ,%hash-table ,hash-table)
+                                 (,updater$a ,key ,val (,copy-rec set ,%hash-table ,hash-table)))))
+             :hints
+             (("Goal"
+               :induct (,copy-rec set ,%hash-table ,hash-table)
+               :in-theory (enable set::subset
+                                  set::in
+                                  ,hash-table$a-theorems
+                                  ,hash-table$a-aggressive)
+               :expand (:free (,key ,val)
+                              (,copy-rec set (,updater$a ,key ,val ,%hash-table) ,hash-table))))))
+
+         (local
+           (defthmd ,copy-rec-of-updater$a-3
+             (implies (and (,keys$ap set)
+                           (not (set::in ,(if key-fixer `(,key-fixer ,key) key) set)))
+                      (equal (,copy-rec set ,%hash-table (,updater$a ,key ,val ,hash-table))
+                             (,copy-rec set ,%hash-table ,hash-table)))
+             :hints
+             (("Goal"
+               :induct (,copy-rec set ,%hash-table ,hash-table)
+               :in-theory (enable set::subset
+                                  set::in
+                                  ,hash-table$a-theorems
+                                  ,hash-table$a-aggressive
+                                  ,copy-rec-of-updater$a-2)
+               :expand (:free (,key ,val)
+                              (,copy-rec set ,%hash-table (,updater$a ,key ,val ,hash-table)))))))
+
+         (local
+           (defthmd ,copy-rec-of-fixer$a-3
+             (equal (,copy-rec set ,%hash-table (,fixer$a ,hash-table))
+                    (,copy-rec set ,%hash-table ,hash-table))
+             :hints
+             (("Goal"
+               :induct (,copy-rec set ,%hash-table ,hash-table)
+               :in-theory (enable ,hash-table$a-theorems
+                                  ,hash-table$a-aggressive)
+               :expand (,copy-rec set ,%hash-table (,fixer$a ,hash-table))))))
+
+         (defthm ,hash-table-copy-constraints
+           (and (equal (,copy-rec set ,%hash-table ,hash-table)
+                       (if (if (set::emptyp set)
+                               (set::emptyp set)
+                               (not (,keys$ap set)))
+                           (,fixer$a ,%hash-table)
+                           ((lambda (,key ,%hash-table set ,hash-table)
+                              ((lambda (,val ,hash-table set ,%hash-table ,key)
+                                 ((lambda (,%val ,key ,%hash-table set ,hash-table ,val)
+                                    (declare (ignorable ,%val))
+                                    ((lambda (,%val ,val ,hash-table set ,%hash-table ,key)
+                                       ((lambda (,%hash-table set ,hash-table ,val ,key)
+                                          ((lambda (,hash-table ,%hash-table set)
+                                             (,copy-rec (set::tail set) ,%hash-table ,hash-table))
+                                           (,updater$a ,key ,val ,hash-table)
+                                           ,%hash-table set))
+                                        (,updater$a ,key ,%val ,%hash-table)
+                                        set ,hash-table ,val ,key))
+                                     ,(cond
+                                        (val-copy
+                                         `(,val-copy ,%val ,val))
+                                        (val-fixer
+                                         `(,val-fixer ,val))
+                                        (t
+                                         val))
+                                     ,val ,hash-table set ,%hash-table ,key))
+                                  (,accessor$a ,key ,%hash-table)
+                                  ,key ,%hash-table set ,hash-table ,val))
+                               (,accessor$a ,key ,hash-table)
+                               ,hash-table set ,%hash-table ,key))
+                            (set::head set)
+                            ,%hash-table set ,hash-table)))
+                (equal (,copy ,%hash-table ,hash-table)
+                       ((lambda (,keys$a ,%hash-table ,hash-table)
+                          ((lambda (count ,keys$a ,hash-table ,%hash-table)
+                             ((lambda (,%hash-table ,hash-table ,keys$a)
+                                ((lambda (,%hash-table ,hash-table ,keys$a)
+                                   (,copy-rec ,keys$a ,%hash-table ,hash-table))
+                                 (,keys$a-set ,keys$a ,%hash-table)
+                                 ,hash-table ,keys$a))
+                              (,init$a count 'nil 'nil ,%hash-table)
+                              ,hash-table ,keys$a))
+                           (,count$a ,hash-table)
+                           ,keys$a
+                           ,hash-table ,%hash-table))
+                        (,keys$a ,hash-table)
+                        ,%hash-table ,hash-table)))
+           :rule-classes
+           ((:definition :corollary
+                (equal (,copy-rec set ,%hash-table ,hash-table)
+                       (if (if (set::emptyp set)
+                               (set::emptyp set)
+                               (not (,keys$ap set)))
+                           (,fixer$a ,%hash-table)
+                           ((lambda (,key ,%hash-table set ,hash-table)
+                              ((lambda (,val ,hash-table set ,%hash-table ,key)
+                                 ((lambda (,%val ,key ,%hash-table set ,hash-table ,val)
+                                    (declare (ignorable ,%val))
+                                    ((lambda (,%val ,val ,hash-table set ,%hash-table ,key)
+                                       ((lambda (,%hash-table set ,hash-table ,val ,key)
+                                          ((lambda (,hash-table ,%hash-table set)
+                                             (,copy-rec (set::tail set) ,%hash-table ,hash-table))
+                                           (,updater$a ,key ,val ,hash-table)
+                                           ,%hash-table set))
+                                        (,updater$a ,key ,%val ,%hash-table)
+                                        set ,hash-table ,val ,key))
+                                     ,(cond
+                                        (val-copy
+                                         `(,val-copy ,%val ,val))
+                                        (val-fixer
+                                         `(,val-fixer ,val))
+                                        (t
+                                         val))
+                                     ,val ,hash-table set ,%hash-table ,key))
+                                  (,accessor$a ,key ,%hash-table)
+                                  ,key ,%hash-table set ,hash-table ,val))
+                               (,accessor$a ,key ,hash-table)
+                               ,hash-table set ,%hash-table ,key))
+                            (set::head set)
+                            ,%hash-table set ,hash-table)))
+              )
+            (:definition :corollary
+                (equal (,copy ,%hash-table ,hash-table)
+                       ((lambda (,keys$a ,%hash-table ,hash-table)
+                          ((lambda (count ,keys$a ,hash-table ,%hash-table)
+                             ((lambda (,%hash-table ,hash-table ,keys$a)
+                                ((lambda (,%hash-table ,hash-table ,keys$a)
+                                   (,copy-rec ,keys$a ,%hash-table ,hash-table))
+                                 (,keys$a-set ,keys$a ,%hash-table)
+                                 ,hash-table ,keys$a))
+                              (,init$a count 'nil 'nil ,%hash-table)
+                              ,hash-table ,keys$a))
+                           (,count$a ,hash-table)
+                           ,keys$a
+                           ,hash-table ,%hash-table))
+                        (,keys$a ,hash-table)
+                        ,%hash-table ,hash-table))))
+           :hints
+           (("Goal"
+             :do-not-induct t
+             :in-theory (enable ,hash-table$a-theorems
+                                ,hash-table$a-aggressive
+                                ,copy-rec-of-fixer$a-3
+                                ,copy-rec-of-updater$a-3
+                                ,copy-rec-of-updater$a-2)
+             :expand (,copy-rec set ,%hash-table ,hash-table))))
+
+         (local
+           (in-theory
+             (disable ,copy-rec
+                      ,copy)))
+
          (defthm ,recognizer$a-of-copy
            (,recognizer$a (,copy ,%hash-table ,hash-table))
            :hints
            (("Goal"
              :do-not-induct t
+             :in-theory (enable ,hash-table$a-theorems)
              :by (:functional-instance
                   lem-hash-table$a::recognizer/copyable-of-copy
-                  ,@fi-bindings-with-copy))))
+                  ,@fi-bindings-with-copy)
+             :expand ((,copy-rec lem-hash-table$a::set
+                                 lem-hash-table$a::%hash-table
+                                 lem-hash-table$a::hash-table)))))
 
          (defthm ,copy-ignores-1
            (equal (,copy ,%hash-table ,hash-table)
@@ -1490,13 +1684,113 @@
                   lem-hash-table$a::copy-ignores-1
                   ,@fi-bindings-with-copy))))
 
-         (defthm ,copy-of-fixer$a-2
-           (equal (,copy ,%hash-table (,fixer$a ,hash-table))
-                  (,copy ,%hash-table ,hash-table))
+         (defcong ,equiv$a equal (,copy ,%hash-table ,hash-table) 2
            :hints
            (("Goal"
              :by (:functional-instance
-                  lem-hash-table$a::copy-of-fixer/copyable-2
+                  lem-hash-table$a::equiv/copyable-implies-equal-copy-2
+                  ,@fi-bindings-with-copy))))
+
+         (defthm ,coupledp-of-copy
+           (,coupledp (,copy ,%hash-table ,hash-table))
+           :hints
+           (("Goal"
+             :by (:functional-instance
+                  lem-hash-table$a::coupledp-of-copy
+                  ,@fi-bindings-with-copy))))
+
+         (local
+           (defthmd ,accessor$a-of-copy-lemma
+             (equal (,accessor$a ,key (,copy ,%hash-table ,hash-table))
+                    (if (set::in ,(if key-fixer `(,key-fixer ,key) key) (,keys$a ,hash-table))
+                        ,(cond
+                           (val-copy
+                            `(,val-copy ,default-val (,accessor$a ,key ,hash-table)))
+                           (val-fixer
+                            `(,val-fixer (,accessor$a ,key ,hash-table)))
+                           (t
+                            `(,accessor$a ,key ,hash-table)))
+                        ,default-val))
+             :hints
+             (("Goal"
+               :by (:functional-instance
+                    lem-hash-table$a::accessor/copyable-of-copy
+                    ,@fi-bindings-with-copy)))))
+
+         (defthm ,accessor$a-of-copy
+           (equal (,accessor$a ,key (,copy ,%hash-table ,hash-table))
+                  (if (set::in ,(if key-fixer `(,key-fixer ,key) key) (,keys$a ,hash-table))
+                      ,(if val-copy
+                           `(,val-copy ,default-val (,accessor$a ,key ,hash-table))
+                           `(,accessor$a ,key ,hash-table))
+                      ,default-val))
+           :hints
+           (("Goal"
+             :use ,accessor$a-of-copy-lemma)))
+
+         (local
+           (defthmd ,copy-of-updater$a-lemma
+             (equal (,copy ,%hash-table (,updater$a ,key ,val ,hash-table))
+                    (if (set::in ,(if key-fixer `(,key-fixer ,key) key) (,keys$a ,hash-table))
+                        (,updater$a ,key
+                                    ,(cond
+                                       (val-copy
+                                        `(,val-copy ,default-val ,val))
+                                       (val-fixer
+                                        `(,val-fixer ,val))
+                                       (t
+                                        val))
+                                    (,copy ,%hash-table ,hash-table))
+                        (,copy ,%hash-table ,hash-table)))
+             :hints
+             (("Goal"
+               :by (:functional-instance
+                    lem-hash-table$a::copy-of-updater/copyable
+                    ,@fi-bindings-with-copy)))))
+
+         (defthm ,copy-of-updater$a
+           (equal (,copy ,%hash-table (,updater$a ,key ,val ,hash-table))
+                  (if (set::in ,(if key-fixer `(,key-fixer ,key) key) (,keys$a ,hash-table))
+                      (,updater$a ,key
+                                  ,(if val-copy
+                                       `(,val-copy ,default-val ,val)
+                                       val)
+                                  (,copy ,%hash-table ,hash-table))
+                      (,copy ,%hash-table ,hash-table)))
+           :hints
+           (("Goal"
+             :in-theory (enable ,hash-table$a-aggressive)
+             :use ,copy-of-updater$a-lemma)))
+
+         (defthm ,boundp$a-of-copy
+           (equal (,boundp$a ,key (,copy ,%hash-table ,hash-table))
+                  (set::in ,(if key-fixer `(,key-fixer ,key) key) (,keys$a ,hash-table)))
+           :hints
+           (("Goal"
+             :by (:functional-instance
+                  lem-hash-table$a::boundp/copyable-of-copy
+                  ,@fi-bindings-with-copy))))
+
+         (defthm ,copy-of-remover$a
+           (equal (,copy ,%hash-table (,remover$a ,key ,hash-table))
+                  (if (set::in ,(if key-fixer `(,key-fixer ,key) key) (,keys$a ,hash-table))
+                      (,updater$a ,key
+                                  ,default-val
+                                  (,copy ,%hash-table ,hash-table))
+                      (,copy ,%hash-table ,hash-table)))
+           :hints
+           (("Goal"
+             :by (:functional-instance
+                  lem-hash-table$a::copy-of-remover/copyable
+                  ,@fi-bindings-with-copy))))
+
+         (defthm ,count$a-of-copy
+           (equal (,count$a (,copy ,%hash-table ,hash-table))
+                  (set::cardinality (,keys$a ,hash-table)))
+           :hints
+           (("Goal"
+             :by (:functional-instance
+                  lem-hash-table$a::count/copyable-of-copy
                   ,@fi-bindings-with-copy))))
 
          (defthm ,keys$a-of-copy
@@ -1507,9 +1801,6 @@
              :by (:functional-instance
                   lem-hash-table$a::keys-of-copy
                   ,@fi-bindings-with-copy))))
-
-         (in-theory
-           (disable ,copy))
 
          (defthm ,copy-rw
            (implies (,coupledp ,hash-table)
@@ -1524,8 +1815,21 @@
        (deflabel ,copy-end)
 
        (deftheory-static ,copy-theory
-         (set-difference-theories (current-theory ',copy-end)
-                                  (current-theory ',copy-begin))))))
+         (set-difference-theories
+          (set-difference-theories (current-theory ',copy-end)
+                                   (current-theory ',copy-begin))
+          '(,@(and val-coupled-p
+                   `(,coupled-vals-p))
+            ,coupled-keys-p
+            ,coupledp
+            ,coupledp-constraints
+            ,copy-rec
+            ,copy
+            ,hash-table-copy-constraints)))
+
+       (in-theory
+         (union-theories (current-theory ',copy-begin)
+                         (theory ',copy-theory))))))
 
 
 ;;;; `MAKE-FRAME-COPY-EVENTS'
@@ -1537,13 +1841,13 @@
                   :verify-guards nil))
   (let* ((%frame (symbolicate package-witness "%" frame))
          (copy (symbolicate package-witness frame "-COPY"))
-         (copy-rw (symbolicate package-witness copy "-RW"))
 
          (coupledp (symbolicate package-witness frame "-COUPLED-P"))
 
          ;; `FRAME'
          (stobj-property (getpropc frame 'acl2::stobj))
          (recognizer (caadr stobj-property))
+         (the-frame (symbolicate frame "THE-" frame))
 
          ;; `FRAME$A'
          (world (w state))
@@ -1556,9 +1860,12 @@
          (recognizer$a (first (second stobj$a-property)))
          (creator$a (second (second stobj$a-property)))
          (fixer$a (third (second stobj$a-property)))
+         (equiv$a (fourth (second stobj$a-property)))
 
          (fields (first (third stobj$a-property)))
-         (stobjs (fifth (third stobj$a-property)))
+         (%fields (loop$ :for field :in fields
+                        :collect (symbolicate field "%" field)))
+         (stobjs (sixth (third stobj$a-property)))
          (stobj-property-list (loop$ :for stobj :in stobjs
                                     :collect (and (symbolp stobj)
                                                   (getprop stobj
@@ -1590,8 +1897,9 @@
                                               `(,creator$a)
                                               initial-element-name)))
          (fixers$a (fourth (third stobj$a-property)))
-         (accessors$a (sixth (third stobj$a-property)))
-         (view$a (first (eighth (third stobj$a-property))))
+         (equivs$a (fifth (third stobj$a-property)))
+         (accessors$a (seventh (third stobj$a-property)))
+         (view$a (first (ninth (third stobj$a-property))))
 
          ;; Adjust for nested stobj interface shuffle
          (stobj-count (len (remove nil stobjs)))
@@ -1662,13 +1970,16 @@
          (copy-theory (symbolicate package-witness copy "-THEORY"))
 
          ;; Theorem Names
+         (coupledp-tp (symbolicate package-witness coupledp "-TP"))
          (coupledp-when-not-recognizer$a (symbolicate package-witness coupledp "-WHEN-NOT-" recognizer$a))
          (coupledp-of-creator$a (symbolicate package-witness coupledp "-OF-" creator$a))
-         (coupledp-of-fixer$a (symbolicate package-witness coupledp "-OF-" fixer$a))
          (coupledp-of-view$a (symbolicate package-witness coupledp "-OF-" view$a))
 
          (recognizer$a-of-copy (symbolicate package-witness recognizer$a "-OF-" copy))
-         (copy-ignores-1 (symbolicate package-witness copy "-IGNORES-1")))
+         (copy-ignores-1 (symbolicate package-witness copy "-IGNORES-1"))
+         (coupledp-of-copy (symbolicate package-witness coupledp "-OF-" copy))
+         (copy-of-view$a (symbolicate package-witness copy "-OF-" view$a))
+         (copy-rw (symbolicate package-witness copy "-RW")))
 
     `(progn
        (deflabel ,copy-begin)
@@ -1680,33 +1991,44 @@
 
          ,@(loop$ :for recognizer$a :in recognizers$a
                  :as initial-element :in initial-elements
+                 :as initial-element-name :in initial-element-names
                  :as fixer$a :in fixers$a
+                 :as equiv$a :in equivs$a
                  :as field :in fields
-                 :as i :from 0 :to (1- (len fields))
+                 :as %field :in %fields
+                 :as i :from 1 :to (len fields)
                  :when (and recognizer$a
                             fixer$a)
                  :append (list
                           `(local
-                             (defthm ,(symbolicate "ATOMIC-STOBJS" "BOOLEANP-OF-" recognizer$a "-" i)
-                               (booleanp (,recognizer$a ,field))
+                             (defthm ,(symbolicate "ATOMIC-STOBJS" recognizer$a "-CONSTRAINT-" i)
+                               (and (booleanp (,recognizer$a ,field))
+                                    (,recognizer$a ,initial-element))
                                :rule-classes
-                               (:rewrite
-                                :type-prescription)))
+                               ((:rewrite :corollary
+                                          (booleanp (,recognizer$a ,field)))
+                                ,@(and (not (equal initial-element initial-element-name))
+                                       `((:rewrite :corollary
+                                                   (,recognizer$a ,initial-element)))))))
 
                           `(local
-                             (defthm ,(symbolicate "ATOMIC-STOBJS" recognizer$a "-OF-INITIAL-ELEMENT-" i)
-                               (,recognizer$a ,initial-element)
-                               :rule-classes nil))
-
-                          `(local
-                             (defthm ,(symbolicate "ATOMIC-STOBJS" fixer$a "-RW-" i)
+                             (defthm ,(symbolicate "ATOMIC-STOBJS" fixer$a "-CONSTRAINT-" i)
                                (equal (,fixer$a ,field)
                                       (if (,recognizer$a ,field)
                                           ,field
-                                          ,initial-element))))))
+                                          ,initial-element))))
+
+                          `(local
+                             (defthm ,(symbolicate "ATOMIC-STOBJS" equiv$a "-CONSTRAINT-" i)
+                               (equal (,equiv$a ,%field ,field)
+                                      (equal (,fixer$a ,%field)
+                                             (,fixer$a ,field)))))))
 
          (local
            (deflabel prologue-end))
+
+         (local
+           (table acl2::theory-invariant-table nil nil :clear))
 
          (local
            (in-theory
@@ -1716,34 +2038,20 @@
               (set-difference-theories (current-theory 'prologue-end)
                                        (current-theory 'prologue-begin)))))
 
-         ,@(loop$ :for recognizer$a :in recognizers$a
-                 :as fixer$a :in fixers$a
-                 :when (and recognizer$a
-                            fixer$a)
-                 :collect `(local
-                             (in-theory
-                               (e/d ((:e ,recognizer$a)
-                                     (:e ,fixer$a))
-                                    (,recognizer$a
-                                     ,fixer$a)))))
-
-         ,@(loop$ :for stobj$a-property :in stobj$a-property-list
-                 :as creator$a :in creators$a
-                 :when stobj$a-property
-                 :collect `(local
-                             (in-theory
-                               (disable ,creator$a))))
-
-         ,@(loop$ :for stobj-property :in stobj-property-list
-                 :as stobj-copy-theory :in stobj-copy-theory-list
-                 :when stobj-property
+         ,@(loop$ :for stobj-copy-theory :in stobj-copy-theory-list
+                 :when stobj-copy-theory
                  :collect `(local
                              (in-theory
                                (enable ,stobj-copy-theory))))
 
-         ,@(loop$ :for stobj-property :in stobj-property-list
-                 :as absstobj-info :in absstobj-info-list
-                 :when stobj-property
+         ,@(loop$ :for recognizer$a :in recognizers$a
+                 :when recognizer$a
+                 :collect `(local
+                             (in-theory
+                               (enable (:e ,recognizer$a)))))
+
+         ,@(loop$ :for absstobj-info :in absstobj-info-list
+                 :when absstobj-info
                  :collect `(local
                              (in-theory
                                (enable ,@(strip-cars (cdr absstobj-info))))))
@@ -1755,10 +2063,6 @@
          (define-congruent ,frame
            :package-witness ,package-witness
            :debug ,debug)
-
-         (local
-           (in-theory
-             (enable ,@(strip-cars (cdr (getpropc %frame 'acl2::absstobj-info))))))
 
          ;; `COUPLEDP'
          ,@(and (remove nil stobj-coupled-p-list)
@@ -1775,6 +2079,10 @@
 
                   (table coupledp ',frame ',coupledp)
 
+                  (defthm ,coupledp-tp
+                    (booleanp (,coupledp ,frame))
+                    :rule-classes :type-prescription)
+
                   (defthm ,coupledp-when-not-recognizer$a
                     (implies (not (,recognizer$a ,frame))
                              (,coupledp ,frame))
@@ -1785,12 +2093,10 @@
                   (defthm ,coupledp-of-creator$a
                     (,coupledp (,creator$a)))
 
-                  (defthm ,coupledp-of-fixer$a
-                    (equal (,coupledp (,fixer$a ,frame))
-                           (,coupledp ,frame)))
+                  (defcong ,equiv$a equal (,coupledp ,frame) 1)
 
                   (defthm ,coupledp-of-view$a
-                    (equal (,coupledp (,view$a ,@fields ,frame))
+                    (equal (,coupledp (,view$a ,@fields))
                            ,(let ((constraints (loop$ :for stobj-coupled-p :in stobj-coupled-p-list
                                                      :as field :in fields
                                                      :when stobj-coupled-p
@@ -1803,16 +2109,17 @@
                           :as stobj-coupled-p :in stobj-coupled-p-list
                           :when stobj-coupled-p
                           :collect `(defthm ,(symbolicate package-witness stobj-coupled-p "-OF-" accessor$a)
-                                      (implies (coupledp ,frame)
+                                      (implies (,coupledp ,frame)
                                                (,stobj-coupled-p (,accessor$a ,frame)))))
 
-                  (in-theory
-                    (disable ,coupledp))))
+                  (local
+                    (in-theory
+                      (disable ,coupledp)))))
 
          ;; `COPY'
          (defun ,copy (,%frame ,frame)
            (declare (xargs :stobjs (,%frame ,frame)))
-           ,(loop$ :with body := %frame
+           ,(loop$ :with body := `(,the-frame ,%frame)
                   :with fields := (reverse fields)
                   :with stobjs := (reverse stobjs)
                   :with %stobjs := (reverse %stobjs)
@@ -1865,18 +2172,44 @@
                     (equal (,copy ,%frame ,frame)
                            (,copy (,creator$a) ,frame))))
 
+         (defcong ,equiv$a equal (,copy ,%frame ,frame) 2)
+
+         ,@(and (remove nil stobj-coupled-p-list)
+                `((defthm ,coupledp-of-copy
+                    (,coupledp (,copy ,%frame ,frame)))))
+
          ,@(loop$ :for accessor$a :in accessors$a
+                 :as stobj-copy :in stobj-copy-list
+                 :as initial-element :in initial-elements
                  :collect `(local
                              (defthm ,(symbolicate package-witness accessor$a "-OF-" copy)
-                               ,(if (remove nil stobj-coupled-p-list)
-                                    `(implies (,coupledp ,frame)
-                                              (equal (,accessor$a (,copy ,%frame ,frame))
-                                                     (,accessor$a ,frame)))
-                                    `(equal (,accessor$a (,copy ,%frame ,frame))
-                                            (,accessor$a ,frame))))))
+                               (equal (,accessor$a (,copy ,%frame ,frame))
+                                      ,(if stobj-copy
+                                           `(,stobj-copy ,initial-element (,accessor$a ,frame))
+                                           `(,accessor$a ,frame))))))
 
-         (in-theory
-           (disable ,copy))
+         (defthm ,copy-of-view$a
+           (equal (,copy ,frame (,view$a ,@fields))
+                  (,view$a ,@(loop$ :for field :in fields
+                                   :as stobj-copy :in stobj-copy-list
+                                   :as initial-element :in initial-elements
+                                   :collect (if stobj-copy
+                                                `(,stobj-copy ,initial-element ,field)
+                                                field))))
+           :hints
+           (("Goal"
+             :use ((:instance ,frame$a-equal
+                              (,%frame$a (,copy ,frame (,view$a ,@fields)))
+                              (,frame$a (,view$a ,@(loop$ :for field :in fields
+                                                         :as stobj-copy :in stobj-copy-list
+                                                         :as initial-element :in initial-elements
+                                                         :collect (if stobj-copy
+                                                                      `(,stobj-copy ,initial-element ,field)
+                                                                      field)))))))))
+
+         (local
+           (in-theory
+             (disable ,copy)))
 
          (defthm ,copy-rw
            ,(if (remove nil stobj-coupled-p-list)
@@ -1895,8 +2228,16 @@
        (deflabel ,copy-end)
 
        (deftheory-static ,copy-theory
-         (set-difference-theories (current-theory ',copy-end)
-                                  (current-theory ',copy-begin))))))
+         (set-difference-theories
+          (set-difference-theories (current-theory ',copy-end)
+                                   (current-theory ',copy-begin))
+          '(,@(and (remove nil stobj-coupled-p-list)
+                   `(,coupledp))
+            ,copy)))
+
+       (in-theory
+         (union-theories (current-theory ',copy-begin)
+                         (theory ',copy-theory))))))
 
 
 ;;;; `DEFINE-COPY'
