books/projects/atomic-stobjs/constructors/vector.lisp
@@ -57,6 +57,7 @@
 
        (recognizer 'nil)
        (creator 'nil)
+       (fixer 'nil)
        (length 'nil)
        (resizer 'nil)
        (accessor 'nil)
@@ -87,6 +88,7 @@
                               (booleanp executable)
                               (symbol-listp (list recognizer
                                                   creator
+                                                  fixer
                                                   length
                                                   resizer
                                                   accessor
@@ -125,6 +127,7 @@
 
               (recognizer ',recognizer)
               (creator ',creator)
+              (fixer ',fixer)
               (length ',length)
               (resizer ',resizer)
               (accessor ',accessor)
@@ -140,10 +143,12 @@
                               (symbolicate package-witness vector (make-predicate-suffix vector))))
               (creator (or creator
                            (symbolicate package-witness "CREATE-" vector)))
+              (fixer (or fixer
+                         (symbolicate package-witness vector "-FIX")))
               (length (or length
-                          (symbolicate package-witness vector "-LENGTH")))
+                          (symbolicate package-witness vector "-LEN")))
               (resizer (or resizer
-                           (symbolicate package-witness vector "-RESIZE")))
+                           (symbolicate package-witness vector "-RSZ")))
               (accessor (or accessor
                             (symbolicate package-witness vector "-REF")))
               (updater (or updater
@@ -201,6 +206,7 @@
               :exec ,vector$c
               :recognizer ,recognizer
               :creator ,creator
+              :fixer ,fixer
               :length ,length
               :resizer ,resizer
               :accessor ,accessor
@@ -210,6 +216,11 @@
               ,@(and ,package-witness-supplied-p
                      `(:package-witness ,package-witness))
               :debug ,debug)
+
+            (defmacro ,(symbolicate package-witness "THE-" vector) (,vector)
+              (declare (xargs :guard (symbolp ,vector)))
+              `(mbe :logic ,(list ',fixer ,vector)
+                    :exec ,,vector))
 
             (in-theory
               (disable ,(symbolicate (if ,package-witness-supplied-p
